<?xml version="1.0"?>
<rdf:RDF xmlns="http://ontology.decidim.org/decidim_roadmap/"
     xml:base="http://ontology.decidim.org/decidim_roadmap/"
     xmlns:rdf="http://www.w3.org/1999/02/22-rdf-syntax-ns#"
     xmlns:owl="http://www.w3.org/2002/07/owl#"
     xmlns:xml="http://www.w3.org/XML/1998/namespace"
     xmlns:xsd="http://www.w3.org/2001/XMLSchema#"
     xmlns:rdfs="http://www.w3.org/2000/01/rdf-schema#">
    <owl:Ontology rdf:about="http://ontology.decidim.org/decidim_roadmap/">
        <owl:versionIRI rdf:resource="http://ontology.decidim.org/decidim_roadmap/1.0.0"/>
        <rdfs:comment xml:lang="en">OWL ontology for participatory democracy in Decidim.

It provides a formal definition of the types, properties, and interrelationships of the entities that constitute the socio-technical ecosystem of participative democracy in the context of the Decidim platform.

The ontology is formalized and written using the machine-processable language RDF/OWL (Web Ontology Language) for knowledge representation.

This version of the ontology describes not only the current functionalities of Decidim, but also the functionalitites under development and foreseen in the development roadmap.</rdfs:comment>
        <owl:versionInfo xml:lang="en">1.0.0</owl:versionInfo>
        <rdfs:label xml:lang="en">Decidim Ontology</rdfs:label>
    </owl:Ontology>
    


    <!-- 
    ///////////////////////////////////////////////////////////////////////////////////////
    //
    // Object Properties
    //
    ///////////////////////////////////////////////////////////////////////////////////////
     -->

    


    <!-- http://ontology.decidim.org/decidim_roadmap/acts_on -->

    <owl:ObjectProperty rdf:about="http://ontology.decidim.org/decidim_roadmap/acts_on">
        <owl:inverseOf rdf:resource="http://ontology.decidim.org/decidim_roadmap/has_actor"/>
        <rdfs:domain rdf:resource="http://ontology.decidim.org/decidim_roadmap/#Agent"/>
        <rdfs:comment xml:lang="en">General property that defines the relationship between an Agent and an entity on which it perform some action.

Inverse property of has_actor and it has domain Agent.</rdfs:comment>
        <rdfs:label xml:lang="en">acts on</rdfs:label>
    </owl:ObjectProperty>
    


    <!-- http://ontology.decidim.org/decidim_roadmap/administrator_of -->

    <owl:ObjectProperty rdf:about="http://ontology.decidim.org/decidim_roadmap/administrator_of">
        <rdfs:subPropertyOf rdf:resource="http://ontology.decidim.org/decidim_roadmap/acts_on"/>
        <owl:inverseOf rdf:resource="http://ontology.decidim.org/decidim_roadmap/has_administrator"/>
        <rdfs:domain rdf:resource="http://ontology.decidim.org/decidim_roadmap/#RegisteredParticipant"/>
        <rdfs:range rdf:resource="http://ontology.decidim.org/decidim_roadmap/ParticipationArtifact"/>
        <rdfs:label xml:lang="en">administrator of</rdfs:label>
    </owl:ObjectProperty>
    


    <!-- http://ontology.decidim.org/decidim_roadmap/amendment_of -->

    <owl:ObjectProperty rdf:about="http://ontology.decidim.org/decidim_roadmap/amendment_of">
        <rdfs:subPropertyOf rdf:resource="http://ontology.decidim.org/decidim_roadmap/refers_to"/>
        <owl:inverseOf rdf:resource="http://ontology.decidim.org/decidim_roadmap/has_amendment"/>
        <rdf:type rdf:resource="http://www.w3.org/2002/07/owl#FunctionalProperty"/>
        <rdfs:domain rdf:resource="http://ontology.decidim.org/decidim_roadmap/Amendment"/>
        <rdfs:range rdf:resource="http://ontology.decidim.org/decidim_roadmap/Proposal"/>
        <rdfs:label xml:lang="en">amendment of</rdfs:label>
    </owl:ObjectProperty>
    


    <!-- http://ontology.decidim.org/decidim_roadmap/attendee_of -->

    <owl:ObjectProperty rdf:about="http://ontology.decidim.org/decidim_roadmap/attendee_of">
        <rdfs:subPropertyOf rdf:resource="http://ontology.decidim.org/decidim_roadmap/acts_on"/>
        <owl:inverseOf rdf:resource="http://ontology.decidim.org/decidim_roadmap/has_attendee"/>
        <rdfs:domain rdf:resource="http://ontology.decidim.org/decidim_roadmap/RegisteredPerson"/>
        <rdfs:range rdf:resource="http://ontology.decidim.org/decidim_roadmap/Meeting"/>
        <rdfs:label>attendee of</rdfs:label>
    </owl:ObjectProperty>
    


    <!-- http://ontology.decidim.org/decidim_roadmap/belong_to -->

    <owl:ObjectProperty rdf:about="http://ontology.decidim.org/decidim_roadmap/belong_to">
        <owl:inverseOf rdf:resource="http://ontology.decidim.org/decidim_roadmap/includes"/>
        <rdfs:comment xml:lang="en">This general property links an entity to another entity it belongs to.

It is inverse property of property includes.</rdfs:comment>
        <rdfs:label xml:lang="en">belongs to</rdfs:label>
    </owl:ObjectProperty>
    


    <!-- http://ontology.decidim.org/decidim_roadmap/category_of -->

    <owl:ObjectProperty rdf:about="http://ontology.decidim.org/decidim_roadmap/category_of">
        <rdfs:subPropertyOf rdf:resource="http://ontology.decidim.org/decidim_roadmap/specifies"/>
        <owl:inverseOf rdf:resource="http://ontology.decidim.org/decidim_roadmap/has_category"/>
        <rdfs:domain rdf:resource="http://ontology.decidim.org/decidim_roadmap/Category"/>
        <rdfs:range rdf:resource="http://ontology.decidim.org/decidim_roadmap/ParticipationItem"/>
        <rdfs:label xml:lang="en">category of</rdfs:label>
    </owl:ObjectProperty>
    


    <!-- http://ontology.decidim.org/decidim_roadmap/collaborator_of -->

    <owl:ObjectProperty rdf:about="http://ontology.decidim.org/decidim_roadmap/collaborator_of">
        <rdfs:subPropertyOf rdf:resource="http://ontology.decidim.org/decidim_roadmap/acts_on"/>
        <owl:inverseOf rdf:resource="http://ontology.decidim.org/decidim_roadmap/has_collaborator"/>
        <rdfs:domain rdf:resource="http://ontology.decidim.org/decidim_roadmap/#RegisteredParticipant"/>
        <rdfs:range rdf:resource="http://ontology.decidim.org/decidim_roadmap/#RegisteredParticipant"/>
        <rdfs:label xml:lang="en">collaborator of</rdfs:label>
    </owl:ObjectProperty>
    


    <!-- http://ontology.decidim.org/decidim_roadmap/comment_voted_by -->

    <owl:ObjectProperty rdf:about="http://ontology.decidim.org/decidim_roadmap/comment_voted_by">
        <rdfs:subPropertyOf rdf:resource="http://ontology.decidim.org/decidim_roadmap/has_actor"/>
        <owl:inverseOf rdf:resource="http://ontology.decidim.org/decidim_roadmap/votes_comment"/>
        <rdfs:domain rdf:resource="http://ontology.decidim.org/decidim_roadmap/Comment"/>
        <rdfs:range rdf:resource="http://ontology.decidim.org/decidim_roadmap/#RegisteredParticipant"/>
        <rdfs:label>comment voted by</rdfs:label>
    </owl:ObjectProperty>
    


    <!-- http://ontology.decidim.org/decidim_roadmap/configurator_of -->

    <owl:ObjectProperty rdf:about="http://ontology.decidim.org/decidim_roadmap/configurator_of">
        <rdfs:subPropertyOf rdf:resource="http://ontology.decidim.org/decidim_roadmap/belong_to"/>
        <owl:inverseOf rdf:resource="http://ontology.decidim.org/decidim_roadmap/has_configurator"/>
        <rdf:type rdf:resource="http://www.w3.org/2002/07/owl#FunctionalProperty"/>
        <rdfs:domain rdf:resource="http://ontology.decidim.org/decidim_roadmap/Configurator"/>
        <rdfs:range rdf:resource="http://ontology.decidim.org/decidim_roadmap/ParticipationArtifact"/>
        <rdfs:label>configurator of</rdfs:label>
    </owl:ObjectProperty>
    


    <!-- http://ontology.decidim.org/decidim_roadmap/container_of -->

    <owl:ObjectProperty rdf:about="http://ontology.decidim.org/decidim_roadmap/container_of">
        <rdfs:subPropertyOf rdf:resource="http://ontology.decidim.org/decidim_roadmap/includes"/>
        <owl:inverseOf rdf:resource="http://ontology.decidim.org/decidim_roadmap/has_container"/>
        <rdfs:domain rdf:resource="http://ontology.decidim.org/decidim_roadmap/Container"/>
        <rdfs:range rdf:resource="http://ontology.decidim.org/decidim_roadmap/ParticipationItem"/>
        <rdfs:label xml:lang="en">container of</rdfs:label>
    </owl:ObjectProperty>
    


    <!-- http://ontology.decidim.org/decidim_roadmap/creator_of -->

    <owl:ObjectProperty rdf:about="http://ontology.decidim.org/decidim_roadmap/creator_of">
        <rdfs:subPropertyOf rdf:resource="http://ontology.decidim.org/decidim_roadmap/acts_on"/>
        <owl:inverseOf rdf:resource="http://ontology.decidim.org/decidim_roadmap/has_creator"/>
        <rdf:type rdf:resource="http://www.w3.org/2002/07/owl#InverseFunctionalProperty"/>
        <rdfs:domain rdf:resource="http://ontology.decidim.org/decidim_roadmap/#RegisteredParticipant"/>
        <rdfs:range rdf:resource="http://ontology.decidim.org/decidim_roadmap/ParticipationItem"/>
        <rdfs:label>creator of</rdfs:label>
    </owl:ObjectProperty>
    


    <!-- http://ontology.decidim.org/decidim_roadmap/derives -->

    <owl:ObjectProperty rdf:about="http://ontology.decidim.org/decidim_roadmap/derives">
        <rdfs:subPropertyOf rdf:resource="http://ontology.decidim.org/decidim_roadmap/referred_by"/>
        <owl:inverseOf rdf:resource="http://ontology.decidim.org/decidim_roadmap/derives_from"/>
        <rdfs:domain rdf:resource="http://ontology.decidim.org/decidim_roadmap/Result"/>
        <rdfs:range rdf:resource="http://ontology.decidim.org/decidim_roadmap/Project"/>
        <rdfs:label xml:lang="en">derives</rdfs:label>
    </owl:ObjectProperty>
    


    <!-- http://ontology.decidim.org/decidim_roadmap/derives_from -->

    <owl:ObjectProperty rdf:about="http://ontology.decidim.org/decidim_roadmap/derives_from">
        <rdfs:subPropertyOf rdf:resource="http://ontology.decidim.org/decidim_roadmap/refers_to"/>
        <rdfs:domain rdf:resource="http://ontology.decidim.org/decidim_roadmap/Project"/>
        <rdfs:range rdf:resource="http://ontology.decidim.org/decidim_roadmap/Result"/>
        <rdfs:label xml:lang="en">derived from</rdfs:label>
    </owl:ObjectProperty>
    


    <!-- http://ontology.decidim.org/decidim_roadmap/endorser_of -->

    <owl:ObjectProperty rdf:about="http://ontology.decidim.org/decidim_roadmap/endorser_of">
        <rdfs:subPropertyOf rdf:resource="http://ontology.decidim.org/decidim_roadmap/acts_on"/>
        <owl:inverseOf rdf:resource="http://ontology.decidim.org/decidim_roadmap/has_endorser"/>
        <rdfs:domain rdf:resource="http://ontology.decidim.org/decidim_roadmap/#VerifiedParticipant"/>
        <rdfs:range rdf:resource="http://ontology.decidim.org/decidim_roadmap/Proposal"/>
        <rdfs:label xml:lang="en">endorser of</rdfs:label>
    </owl:ObjectProperty>
    


    <!-- http://ontology.decidim.org/decidim_roadmap/first_comment_of -->

    <owl:ObjectProperty rdf:about="http://ontology.decidim.org/decidim_roadmap/first_comment_of">
        <rdfs:subPropertyOf rdf:resource="http://ontology.decidim.org/decidim_roadmap/belong_to"/>
        <owl:inverseOf rdf:resource="http://ontology.decidim.org/decidim_roadmap/has_first_comment"/>
        <rdf:type rdf:resource="http://www.w3.org/2002/07/owl#FunctionalProperty"/>
        <rdfs:domain rdf:resource="http://ontology.decidim.org/decidim_roadmap/FirstLevelComment"/>
        <rdfs:range rdf:resource="http://ontology.decidim.org/decidim_roadmap/Thread"/>
        <rdfs:comment xml:lang="en">By opening a discussion about an Item, a FirstLevelComment starts a Thread. This property associates a FirstLevelComment to the corresponding Thread.</rdfs:comment>
        <rdfs:label>first comment of</rdfs:label>
    </owl:ObjectProperty>
    


    <!-- http://ontology.decidim.org/decidim_roadmap/follower_of -->

    <owl:ObjectProperty rdf:about="http://ontology.decidim.org/decidim_roadmap/follower_of">
        <rdfs:subPropertyOf rdf:resource="http://ontology.decidim.org/decidim_roadmap/acts_on"/>
        <owl:inverseOf rdf:resource="http://ontology.decidim.org/decidim_roadmap/has_follower"/>
        <rdfs:domain rdf:resource="http://ontology.decidim.org/decidim_roadmap/#RegisteredParticipant"/>
        <rdfs:range rdf:resource="http://ontology.decidim.org/decidim_roadmap/ParticipationItem"/>
        <rdfs:comment xml:lang="en">This property associates a RegisteredParticipant to an Item they have subscribed to, in order to receive notifications and updates about it.</rdfs:comment>
        <rdfs:label xml:lang="en">follower of</rdfs:label>
    </owl:ObjectProperty>
    


    <!-- http://ontology.decidim.org/decidim_roadmap/functionality_of -->

    <owl:ObjectProperty rdf:about="http://ontology.decidim.org/decidim_roadmap/functionality_of">
        <rdfs:subPropertyOf rdf:resource="http://ontology.decidim.org/decidim_roadmap/belong_to"/>
        <owl:inverseOf rdf:resource="http://ontology.decidim.org/decidim_roadmap/has_functionality"/>
        <rdfs:domain rdf:resource="http://ontology.decidim.org/decidim_roadmap/#ParticipationSpace"/>
        <rdfs:range rdf:resource="http://ontology.decidim.org/decidim_roadmap/ParticipationFunctionality"/>
        <rdfs:comment xml:lang="en">Indicates that a ParticipationSpace includes a ParticipationFunctionality. 
Each ParticipationSpace can include more instances of the same kind of functionality; for example, a Process may include various Debates and Pages.</rdfs:comment>
        <rdfs:label>functionality of</rdfs:label>
    </owl:ObjectProperty>
    


    <!-- http://ontology.decidim.org/decidim_roadmap/granted_by -->

    <owl:ObjectProperty rdf:about="http://ontology.decidim.org/decidim_roadmap/granted_by">
        <rdfs:subPropertyOf rdf:resource="http://ontology.decidim.org/decidim_roadmap/has_actor"/>
        <owl:inverseOf rdf:resource="http://ontology.decidim.org/decidim_roadmap/grants"/>
        <rdfs:domain rdf:resource="http://ontology.decidim.org/decidim_roadmap/Role"/>
        <rdfs:range rdf:resource="http://ontology.decidim.org/decidim_roadmap/#RegisteredParticipant"/>
        <rdfs:label>granted by</rdfs:label>
    </owl:ObjectProperty>
    


    <!-- http://ontology.decidim.org/decidim_roadmap/grants -->

    <owl:ObjectProperty rdf:about="http://ontology.decidim.org/decidim_roadmap/grants">
        <rdfs:subPropertyOf rdf:resource="http://ontology.decidim.org/decidim_roadmap/acts_on"/>
        <rdfs:domain rdf:resource="http://ontology.decidim.org/decidim_roadmap/#RegisteredParticipant"/>
        <rdfs:range rdf:resource="http://ontology.decidim.org/decidim_roadmap/Role"/>
        <rdfs:label>grants</rdfs:label>
    </owl:ObjectProperty>
    


    <!-- http://ontology.decidim.org/decidim_roadmap/has_actor -->

    <owl:ObjectProperty rdf:about="http://ontology.decidim.org/decidim_roadmap/has_actor">
        <rdfs:range rdf:resource="http://ontology.decidim.org/decidim_roadmap/#Agent"/>
        <rdfs:comment xml:lang="en">general property that defines the relation between an entity and an Agent that performs some action on it.

It is inverse property of acts_on, and it has range Agent.</rdfs:comment>
        <rdfs:label xml:lang="en">has actor</rdfs:label>
    </owl:ObjectProperty>
    


    <!-- http://ontology.decidim.org/decidim_roadmap/has_administrator -->

    <owl:ObjectProperty rdf:about="http://ontology.decidim.org/decidim_roadmap/has_administrator">
        <rdfs:subPropertyOf rdf:resource="http://ontology.decidim.org/decidim_roadmap/has_actor"/>
        <rdfs:domain rdf:resource="http://ontology.decidim.org/decidim_roadmap/ParticipationArtifact"/>
        <rdfs:range rdf:resource="http://ontology.decidim.org/decidim_roadmap/#RegisteredParticipant"/>
        <rdfs:label xml:lang="en">has administrator</rdfs:label>
    </owl:ObjectProperty>
    


    <!-- http://ontology.decidim.org/decidim_roadmap/has_amendment -->

    <owl:ObjectProperty rdf:about="http://ontology.decidim.org/decidim_roadmap/has_amendment">
        <rdfs:subPropertyOf rdf:resource="http://ontology.decidim.org/decidim_roadmap/referred_by"/>
        <rdf:type rdf:resource="http://www.w3.org/2002/07/owl#InverseFunctionalProperty"/>
        <rdfs:domain rdf:resource="http://ontology.decidim.org/decidim_roadmap/Proposal"/>
        <rdfs:range rdf:resource="http://ontology.decidim.org/decidim_roadmap/Amendment"/>
        <rdfs:label>has amendment</rdfs:label>
    </owl:ObjectProperty>
    


    <!-- http://ontology.decidim.org/decidim_roadmap/has_attendee -->

    <owl:ObjectProperty rdf:about="http://ontology.decidim.org/decidim_roadmap/has_attendee">
        <rdfs:subPropertyOf rdf:resource="http://ontology.decidim.org/decidim_roadmap/has_actor"/>
        <rdfs:domain rdf:resource="http://ontology.decidim.org/decidim_roadmap/Meeting"/>
        <rdfs:range rdf:resource="http://ontology.decidim.org/decidim_roadmap/RegisteredPerson"/>
        <rdfs:label xml:lang="en">has attendee</rdfs:label>
    </owl:ObjectProperty>
    


    <!-- http://ontology.decidim.org/decidim_roadmap/has_category -->

    <owl:ObjectProperty rdf:about="http://ontology.decidim.org/decidim_roadmap/has_category">
        <rdfs:subPropertyOf rdf:resource="http://ontology.decidim.org/decidim_roadmap/specified_by"/>
        <rdfs:domain rdf:resource="http://ontology.decidim.org/decidim_roadmap/ParticipationItem"/>
        <rdfs:range rdf:resource="http://ontology.decidim.org/decidim_roadmap/Category"/>
        <rdfs:label xml:lang="en">has category</rdfs:label>
    </owl:ObjectProperty>
    


    <!-- http://ontology.decidim.org/decidim_roadmap/has_collaborator -->

    <owl:ObjectProperty rdf:about="http://ontology.decidim.org/decidim_roadmap/has_collaborator">
        <rdfs:subPropertyOf rdf:resource="http://ontology.decidim.org/decidim_roadmap/has_actor"/>
        <rdfs:domain rdf:resource="http://ontology.decidim.org/decidim_roadmap/ParticipationArtifact"/>
        <rdfs:range rdf:resource="http://ontology.decidim.org/decidim_roadmap/#RegisteredParticipant"/>
        <rdfs:label xml:lang="en">has collaborator</rdfs:label>
    </owl:ObjectProperty>
    


    <!-- http://ontology.decidim.org/decidim_roadmap/has_configurator -->

    <owl:ObjectProperty rdf:about="http://ontology.decidim.org/decidim_roadmap/has_configurator">
        <rdfs:subPropertyOf rdf:resource="http://ontology.decidim.org/decidim_roadmap/includes"/>
        <rdf:type rdf:resource="http://www.w3.org/2002/07/owl#InverseFunctionalProperty"/>
        <rdfs:domain rdf:resource="http://ontology.decidim.org/decidim_roadmap/ParticipationArtifact"/>
        <rdfs:range rdf:resource="http://ontology.decidim.org/decidim_roadmap/Configurator"/>
        <rdfs:label>has configurator</rdfs:label>
    </owl:ObjectProperty>
    


    <!-- http://ontology.decidim.org/decidim_roadmap/has_container -->

    <owl:ObjectProperty rdf:about="http://ontology.decidim.org/decidim_roadmap/has_container">
        <rdfs:subPropertyOf rdf:resource="http://ontology.decidim.org/decidim_roadmap/belong_to"/>
        <rdfs:domain rdf:resource="http://ontology.decidim.org/decidim_roadmap/ParticipationItem"/>
        <rdfs:range rdf:resource="http://ontology.decidim.org/decidim_roadmap/Container"/>
        <rdfs:label xml:lang="en">has container</rdfs:label>
    </owl:ObjectProperty>
    


    <!-- http://ontology.decidim.org/decidim_roadmap/has_creator -->

    <owl:ObjectProperty rdf:about="http://ontology.decidim.org/decidim_roadmap/has_creator">
        <rdfs:subPropertyOf rdf:resource="http://ontology.decidim.org/decidim_roadmap/has_actor"/>
        <rdf:type rdf:resource="http://www.w3.org/2002/07/owl#FunctionalProperty"/>
        <rdfs:domain rdf:resource="http://ontology.decidim.org/decidim_roadmap/ParticipationItem"/>
        <rdfs:range rdf:resource="http://ontology.decidim.org/decidim_roadmap/#RegisteredParticipant"/>
        <rdfs:comment xml:lang="en">This property links an AuthoredItem to its creator.</rdfs:comment>
        <rdfs:label>has creator</rdfs:label>
    </owl:ObjectProperty>
    


    <!-- http://ontology.decidim.org/decidim_roadmap/has_endorser -->

    <owl:ObjectProperty rdf:about="http://ontology.decidim.org/decidim_roadmap/has_endorser">
        <rdfs:subPropertyOf rdf:resource="http://ontology.decidim.org/decidim_roadmap/has_actor"/>
        <rdfs:domain rdf:resource="http://ontology.decidim.org/decidim_roadmap/Proposal"/>
        <rdfs:range rdf:resource="http://ontology.decidim.org/decidim_roadmap/#VerifiedParticipant"/>
        <rdfs:label>has endorser</rdfs:label>
    </owl:ObjectProperty>
    


    <!-- http://ontology.decidim.org/decidim_roadmap/has_first_comment -->

    <owl:ObjectProperty rdf:about="http://ontology.decidim.org/decidim_roadmap/has_first_comment">
        <rdfs:subPropertyOf rdf:resource="http://ontology.decidim.org/decidim_roadmap/includes"/>
        <rdf:type rdf:resource="http://www.w3.org/2002/07/owl#FunctionalProperty"/>
        <rdfs:domain rdf:resource="http://ontology.decidim.org/decidim_roadmap/Thread"/>
        <rdfs:range rdf:resource="http://ontology.decidim.org/decidim_roadmap/FirstLevelComment"/>
        <rdfs:comment xml:lang="en">This property associates a Thread with the FirstLevelComment that opens it.</rdfs:comment>
        <rdfs:label xml:lang="en">has first comment</rdfs:label>
    </owl:ObjectProperty>
    


    <!-- http://ontology.decidim.org/decidim_roadmap/has_follower -->

    <owl:ObjectProperty rdf:about="http://ontology.decidim.org/decidim_roadmap/has_follower">
        <rdfs:subPropertyOf rdf:resource="http://ontology.decidim.org/decidim_roadmap/has_actor"/>
        <rdfs:domain rdf:resource="http://ontology.decidim.org/decidim_roadmap/ParticipationItem"/>
        <rdfs:range rdf:resource="http://ontology.decidim.org/decidim_roadmap/#RegisteredParticipant"/>
        <rdfs:label xml:lang="en">has follower</rdfs:label>
    </owl:ObjectProperty>
    


    <!-- http://ontology.decidim.org/decidim_roadmap/has_functionality -->

    <owl:ObjectProperty rdf:about="http://ontology.decidim.org/decidim_roadmap/has_functionality">
        <rdfs:subPropertyOf rdf:resource="http://ontology.decidim.org/decidim_roadmap/includes"/>
        <rdfs:domain rdf:resource="http://ontology.decidim.org/decidim_roadmap/#ParticipationSpace"/>
        <rdfs:range rdf:resource="http://ontology.decidim.org/decidim_roadmap/ParticipationFunctionality"/>
        <rdfs:label>has functionality</rdfs:label>
    </owl:ObjectProperty>
    


    <!-- http://ontology.decidim.org/decidim_roadmap/has_initiative -->

    <owl:ObjectProperty rdf:about="http://ontology.decidim.org/decidim_roadmap/has_initiative">
        <rdfs:subPropertyOf rdf:resource="http://ontology.decidim.org/decidim_roadmap/belong_to"/>
        <owl:inverseOf rdf:resource="http://ontology.decidim.org/decidim_roadmap/initiative_of"/>
        <rdf:type rdf:resource="http://www.w3.org/2002/07/owl#InverseFunctionalProperty"/>
        <rdfs:domain rdf:resource="http://ontology.decidim.org/decidim_roadmap/Initiative"/>
        <rdfs:range rdf:resource="http://ontology.decidim.org/decidim_roadmap/Proposal"/>
        <rdfs:label>has initiative</rdfs:label>
    </owl:ObjectProperty>
    


    <!-- http://ontology.decidim.org/decidim_roadmap/has_member -->

    <owl:ObjectProperty rdf:about="http://ontology.decidim.org/decidim_roadmap/has_member">
        <rdfs:subPropertyOf rdf:resource="http://ontology.decidim.org/decidim_roadmap/includes"/>
        <owl:inverseOf rdf:resource="http://ontology.decidim.org/decidim_roadmap/member_of"/>
        <rdfs:domain rdf:resource="http://ontology.decidim.org/decidim_roadmap/Group"/>
        <rdfs:range rdf:resource="http://ontology.decidim.org/decidim_roadmap/#RegisteredParticipant"/>
        <rdfs:label xml:lang="en">has member</rdfs:label>
    </owl:ObjectProperty>
    


    <!-- http://ontology.decidim.org/decidim_roadmap/has_moderator -->

    <owl:ObjectProperty rdf:about="http://ontology.decidim.org/decidim_roadmap/has_moderator">
        <rdfs:subPropertyOf rdf:resource="http://ontology.decidim.org/decidim_roadmap/has_actor"/>
        <owl:inverseOf rdf:resource="http://ontology.decidim.org/decidim_roadmap/moderator_of"/>
        <rdfs:domain rdf:resource="http://ontology.decidim.org/decidim_roadmap/ParticipationArtifact"/>
        <rdfs:range rdf:resource="http://ontology.decidim.org/decidim_roadmap/#RegisteredParticipant"/>
        <rdfs:label xml:lang="en">has moderator</rdfs:label>
    </owl:ObjectProperty>
    


    <!-- http://ontology.decidim.org/decidim_roadmap/has_participant -->

    <owl:ObjectProperty rdf:about="http://ontology.decidim.org/decidim_roadmap/has_participant">
        <rdfs:subPropertyOf rdf:resource="http://ontology.decidim.org/decidim_roadmap/has_actor"/>
        <owl:inverseOf rdf:resource="http://ontology.decidim.org/decidim_roadmap/participant_of"/>
        <rdfs:domain rdf:resource="http://ontology.decidim.org/decidim_roadmap/ParticipationArtifact"/>
        <rdfs:range rdf:resource="http://ontology.decidim.org/decidim_roadmap/#Agent"/>
        <rdfs:label xml:lang="en">has participant</rdfs:label>
    </owl:ObjectProperty>
    


    <!-- http://ontology.decidim.org/decidim_roadmap/has_phase -->

    <owl:ObjectProperty rdf:about="http://ontology.decidim.org/decidim_roadmap/has_phase">
        <rdfs:subPropertyOf rdf:resource="http://ontology.decidim.org/decidim_roadmap/includes"/>
        <owl:inverseOf rdf:resource="http://ontology.decidim.org/decidim_roadmap/phase_of"/>
        <rdf:type rdf:resource="http://www.w3.org/2002/07/owl#InverseFunctionalProperty"/>
        <rdfs:domain rdf:resource="http://ontology.decidim.org/decidim_roadmap/Process"/>
        <rdfs:range rdf:resource="http://ontology.decidim.org/decidim_roadmap/Phase"/>
        <rdfs:label xml:lang="en">has phase</rdfs:label>
    </owl:ObjectProperty>
    


    <!-- http://ontology.decidim.org/decidim_roadmap/has_platform -->

    <owl:ObjectProperty rdf:about="http://ontology.decidim.org/decidim_roadmap/has_platform">
        <rdfs:subPropertyOf rdf:resource="http://ontology.decidim.org/decidim_roadmap/belong_to"/>
        <owl:inverseOf rdf:resource="http://ontology.decidim.org/decidim_roadmap/platform_of"/>
        <rdfs:domain rdf:resource="http://ontology.decidim.org/decidim_roadmap/#ParticipationSpace"/>
        <rdfs:range rdf:resource="http://ontology.decidim.org/decidim_roadmap/ParticipationPlatform"/>
        <rdfs:label xml:lang="en">has platform</rdfs:label>
    </owl:ObjectProperty>
    


    <!-- http://ontology.decidim.org/decidim_roadmap/has_promoter -->

    <owl:ObjectProperty rdf:about="http://ontology.decidim.org/decidim_roadmap/has_promoter">
        <rdfs:subPropertyOf rdf:resource="http://ontology.decidim.org/decidim_roadmap/has_actor"/>
        <owl:inverseOf rdf:resource="http://ontology.decidim.org/decidim_roadmap/promoter_of"/>
        <rdfs:domain rdf:resource="http://ontology.decidim.org/decidim_roadmap/#ParticipationSpace"/>
        <rdfs:range rdf:resource="http://ontology.decidim.org/decidim_roadmap/Group"/>
        <rdfs:label xml:lang="en">has promoter</rdfs:label>
        <rdfs:label>promoted by</rdfs:label>
    </owl:ObjectProperty>
    


    <!-- http://ontology.decidim.org/decidim_roadmap/has_reply -->

    <owl:ObjectProperty rdf:about="http://ontology.decidim.org/decidim_roadmap/has_reply">
        <rdfs:subPropertyOf rdf:resource="http://ontology.decidim.org/decidim_roadmap/referred_by"/>
        <owl:inverseOf rdf:resource="http://ontology.decidim.org/decidim_roadmap/reply_of"/>
        <rdfs:domain rdf:resource="http://ontology.decidim.org/decidim_roadmap/ParticipationItem"/>
        <rdfs:range rdf:resource="http://ontology.decidim.org/decidim_roadmap/Comment"/>
        <rdfs:comment xml:lang="en">Points to an Comment that is a reply or response to this Item.</rdfs:comment>
        <rdfs:label xml:lang="en">has reply</rdfs:label>
    </owl:ObjectProperty>
    


    <!-- http://ontology.decidim.org/decidim_roadmap/has_result -->

    <owl:ObjectProperty rdf:about="http://ontology.decidim.org/decidim_roadmap/has_result">
        <rdfs:subPropertyOf rdf:resource="http://ontology.decidim.org/decidim_roadmap/referred_by"/>
        <owl:inverseOf rdf:resource="http://ontology.decidim.org/decidim_roadmap/result_of"/>
        <rdfs:domain rdf:resource="http://ontology.decidim.org/decidim_roadmap/Proposal"/>
        <rdfs:range rdf:resource="http://ontology.decidim.org/decidim_roadmap/Result"/>
        <rdfs:label>has result</rdfs:label>
    </owl:ObjectProperty>
    


    <!-- http://ontology.decidim.org/decidim_roadmap/has_role -->

    <owl:ObjectProperty rdf:about="http://ontology.decidim.org/decidim_roadmap/has_role">
        <rdfs:subPropertyOf rdf:resource="http://ontology.decidim.org/decidim_roadmap/specified_by"/>
        <owl:inverseOf rdf:resource="http://ontology.decidim.org/decidim_roadmap/role_of"/>
        <rdfs:domain rdf:resource="http://ontology.decidim.org/decidim_roadmap/#RegisteredParticipant"/>
        <rdfs:range rdf:resource="http://ontology.decidim.org/decidim_roadmap/Role"/>
        <rdfs:label>has role</rdfs:label>
    </owl:ObjectProperty>
    


    <!-- http://ontology.decidim.org/decidim_roadmap/has_role_scope -->

    <owl:ObjectProperty rdf:about="http://ontology.decidim.org/decidim_roadmap/has_role_scope">
        <rdfs:subPropertyOf rdf:resource="http://ontology.decidim.org/decidim_roadmap/specified_by"/>
        <owl:inverseOf rdf:resource="http://ontology.decidim.org/decidim_roadmap/role_scope_of"/>
        <rdf:type rdf:resource="http://www.w3.org/2002/07/owl#FunctionalProperty"/>
        <rdfs:domain rdf:resource="http://ontology.decidim.org/decidim_roadmap/Role"/>
        <rdfs:range rdf:resource="http://ontology.decidim.org/decidim_roadmap/ParticipationArtifact"/>
        <rdfs:label xml:lang="en">has role scope</rdfs:label>
    </owl:ObjectProperty>
    


    <!-- http://ontology.decidim.org/decidim_roadmap/has_scope -->

    <owl:ObjectProperty rdf:about="http://ontology.decidim.org/decidim_roadmap/has_scope">
        <rdfs:subPropertyOf rdf:resource="http://ontology.decidim.org/decidim_roadmap/specified_by"/>
        <owl:inverseOf rdf:resource="http://ontology.decidim.org/decidim_roadmap/scope_of"/>
        <rdfs:range rdf:resource="http://ontology.decidim.org/decidim_roadmap/Scope"/>
        <rdfs:label xml:lang="en">has scope</rdfs:label>
    </owl:ObjectProperty>
    


    <!-- http://ontology.decidim.org/decidim_roadmap/has_subcategory -->

    <owl:ObjectProperty rdf:about="http://ontology.decidim.org/decidim_roadmap/has_subcategory">
        <rdfs:subPropertyOf rdf:resource="http://ontology.decidim.org/decidim_roadmap/includes"/>
        <owl:inverseOf rdf:resource="http://ontology.decidim.org/decidim_roadmap/subcategory_of"/>
        <rdfs:domain rdf:resource="http://ontology.decidim.org/decidim_roadmap/Category"/>
        <rdfs:range rdf:resource="http://ontology.decidim.org/decidim_roadmap/Category"/>
        <rdfs:label xml:lang="en">has_subcategory</rdfs:label>
    </owl:ObjectProperty>
    


    <!-- http://ontology.decidim.org/decidim_roadmap/has_subgroup -->

    <owl:ObjectProperty rdf:about="http://ontology.decidim.org/decidim_roadmap/has_subgroup">
        <rdfs:subPropertyOf rdf:resource="http://ontology.decidim.org/decidim_roadmap/includes"/>
        <rdfs:domain rdf:resource="http://ontology.decidim.org/decidim_roadmap/Group"/>
        <rdfs:range rdf:resource="http://ontology.decidim.org/decidim_roadmap/Group"/>
        <rdfs:label xml:lang="en">has subgroup</rdfs:label>
    </owl:ObjectProperty>
    


    <!-- http://ontology.decidim.org/decidim_roadmap/has_supporter -->

    <owl:ObjectProperty rdf:about="http://ontology.decidim.org/decidim_roadmap/has_supporter">
        <rdfs:subPropertyOf rdf:resource="http://ontology.decidim.org/decidim_roadmap/has_actor"/>
        <owl:inverseOf rdf:resource="http://ontology.decidim.org/decidim_roadmap/supporter_of"/>
        <rdfs:domain rdf:resource="http://ontology.decidim.org/decidim_roadmap/Proposal"/>
        <rdfs:range rdf:resource="http://ontology.decidim.org/decidim_roadmap/RegisteredPerson"/>
        <rdfs:label xml:lang="en">has supporter</rdfs:label>
    </owl:ObjectProperty>
    


    <!-- http://ontology.decidim.org/decidim_roadmap/includes -->

    <owl:ObjectProperty rdf:about="http://ontology.decidim.org/decidim_roadmap/includes">
        <rdfs:comment xml:lang="en">This general property links an entity to another entity belonging to it.

It is inverse property of belongs_to.</rdfs:comment>
        <rdfs:label xml:lang="en">includes</rdfs:label>
    </owl:ObjectProperty>
    


    <!-- http://ontology.decidim.org/decidim_roadmap/initiative_of -->

    <owl:ObjectProperty rdf:about="http://ontology.decidim.org/decidim_roadmap/initiative_of">
        <rdfs:subPropertyOf rdf:resource="http://ontology.decidim.org/decidim_roadmap/includes"/>
        <rdf:type rdf:resource="http://www.w3.org/2002/07/owl#FunctionalProperty"/>
        <rdfs:domain rdf:resource="http://ontology.decidim.org/decidim_roadmap/Proposal"/>
        <rdfs:range rdf:resource="http://ontology.decidim.org/decidim_roadmap/Initiative"/>
        <rdfs:label>initiative of</rdfs:label>
    </owl:ObjectProperty>
    


    <!-- http://ontology.decidim.org/decidim_roadmap/member_of -->

    <owl:ObjectProperty rdf:about="http://ontology.decidim.org/decidim_roadmap/member_of">
        <rdfs:subPropertyOf rdf:resource="http://ontology.decidim.org/decidim_roadmap/belong_to"/>
        <rdfs:domain rdf:resource="http://ontology.decidim.org/decidim_roadmap/#RegisteredParticipant"/>
        <rdfs:range rdf:resource="http://ontology.decidim.org/decidim_roadmap/Group"/>
        <rdfs:label xml:lang="en">member of</rdfs:label>
    </owl:ObjectProperty>
    


    <!-- http://ontology.decidim.org/decidim_roadmap/mentioned_by -->

    <owl:ObjectProperty rdf:about="http://ontology.decidim.org/decidim_roadmap/mentioned_by">
        <rdfs:subPropertyOf rdf:resource="http://ontology.decidim.org/decidim_roadmap/referred_by"/>
        <owl:inverseOf rdf:resource="http://ontology.decidim.org/decidim_roadmap/mentions"/>
        <rdfs:domain rdf:resource="http://ontology.decidim.org/decidim_roadmap/#RegisteredParticipant"/>
        <rdfs:range rdf:resource="http://ontology.decidim.org/decidim_roadmap/Comment"/>
        <rdfs:label xml:lang="en">mentioned by</rdfs:label>
    </owl:ObjectProperty>
    


    <!-- http://ontology.decidim.org/decidim_roadmap/mentions -->

    <owl:ObjectProperty rdf:about="http://ontology.decidim.org/decidim_roadmap/mentions">
        <rdfs:subPropertyOf rdf:resource="http://ontology.decidim.org/decidim_roadmap/refers_to"/>
        <rdfs:domain rdf:resource="http://ontology.decidim.org/decidim_roadmap/Comment"/>
        <rdfs:range rdf:resource="http://ontology.decidim.org/decidim_roadmap/#RegisteredParticipant"/>
        <rdfs:label xml:lang="en">mentions</rdfs:label>
    </owl:ObjectProperty>
    


    <!-- http://ontology.decidim.org/decidim_roadmap/moderator_of -->

    <owl:ObjectProperty rdf:about="http://ontology.decidim.org/decidim_roadmap/moderator_of">
        <rdfs:subPropertyOf rdf:resource="http://ontology.decidim.org/decidim_roadmap/acts_on"/>
        <rdfs:domain rdf:resource="http://ontology.decidim.org/decidim_roadmap/#RegisteredParticipant"/>
        <rdfs:range rdf:resource="http://ontology.decidim.org/decidim_roadmap/ParticipationArtifact"/>
        <rdfs:label xml:lang="en">moderator of</rdfs:label>
    </owl:ObjectProperty>
    


    <!-- http://ontology.decidim.org/decidim_roadmap/participant_of -->

    <owl:ObjectProperty rdf:about="http://ontology.decidim.org/decidim_roadmap/participant_of">
        <rdfs:subPropertyOf rdf:resource="http://ontology.decidim.org/decidim_roadmap/acts_on"/>
        <rdfs:domain rdf:resource="http://ontology.decidim.org/decidim_roadmap/#Agent"/>
        <rdfs:range rdf:resource="http://ontology.decidim.org/decidim_roadmap/ParticipationArtifact"/>
        <rdfs:label xml:lang="en">participant of</rdfs:label>
    </owl:ObjectProperty>
    


    <!-- http://ontology.decidim.org/decidim_roadmap/phase_of -->

    <owl:ObjectProperty rdf:about="http://ontology.decidim.org/decidim_roadmap/phase_of">
        <rdfs:subPropertyOf rdf:resource="http://ontology.decidim.org/decidim_roadmap/belong_to"/>
        <rdf:type rdf:resource="http://www.w3.org/2002/07/owl#FunctionalProperty"/>
        <rdfs:domain rdf:resource="http://ontology.decidim.org/decidim_roadmap/Phase"/>
        <rdfs:range rdf:resource="http://ontology.decidim.org/decidim_roadmap/Process"/>
        <rdfs:label xml:lang="en">phase of</rdfs:label>
    </owl:ObjectProperty>
    


    <!-- http://ontology.decidim.org/decidim_roadmap/platform_of -->

    <owl:ObjectProperty rdf:about="http://ontology.decidim.org/decidim_roadmap/platform_of">
        <rdfs:subPropertyOf rdf:resource="http://ontology.decidim.org/decidim_roadmap/includes"/>
        <rdfs:domain rdf:resource="http://ontology.decidim.org/decidim_roadmap/ParticipationPlatform"/>
        <rdfs:range rdf:resource="http://ontology.decidim.org/decidim_roadmap/#ParticipationSpace"/>
        <rdfs:label xml:lang="en">platform of</rdfs:label>
    </owl:ObjectProperty>
    


    <!-- http://ontology.decidim.org/decidim_roadmap/promoter_of -->

    <owl:ObjectProperty rdf:about="http://ontology.decidim.org/decidim_roadmap/promoter_of">
        <rdfs:subPropertyOf rdf:resource="http://ontology.decidim.org/decidim_roadmap/acts_on"/>
        <rdfs:domain rdf:resource="http://ontology.decidim.org/decidim_roadmap/Group"/>
        <rdfs:range rdf:resource="http://ontology.decidim.org/decidim_roadmap/#ParticipationSpace"/>
        <rdfs:comment></rdfs:comment>
        <rdfs:label xml:lang="en">promoter of</rdfs:label>
        <rdfs:label>promotes</rdfs:label>
    </owl:ObjectProperty>
    


    <!-- http://ontology.decidim.org/decidim_roadmap/referenced_by -->

    <owl:ObjectProperty rdf:about="http://ontology.decidim.org/decidim_roadmap/referenced_by">
        <rdfs:subPropertyOf rdf:resource="http://ontology.decidim.org/decidim_roadmap/referred_by"/>
        <owl:inverseOf rdf:resource="http://ontology.decidim.org/decidim_roadmap/references"/>
        <rdfs:domain rdf:resource="http://ontology.decidim.org/decidim_roadmap/ParticipationItem"/>
        <rdfs:range rdf:resource="http://ontology.decidim.org/decidim_roadmap/ParticipationItem"/>
        <rdfs:label xml:lang="en">referenced by</rdfs:label>
    </owl:ObjectProperty>
    


    <!-- http://ontology.decidim.org/decidim_roadmap/references -->

    <owl:ObjectProperty rdf:about="http://ontology.decidim.org/decidim_roadmap/references">
        <rdfs:subPropertyOf rdf:resource="http://ontology.decidim.org/decidim_roadmap/refers_to"/>
        <rdfs:domain rdf:resource="http://ontology.decidim.org/decidim_roadmap/ParticipationItem"/>
        <rdfs:range rdf:resource="http://ontology.decidim.org/decidim_roadmap/ParticipationItem"/>
        <rdfs:label>references</rdfs:label>
    </owl:ObjectProperty>
    


    <!-- http://ontology.decidim.org/decidim_roadmap/referred_by -->

    <owl:ObjectProperty rdf:about="http://ontology.decidim.org/decidim_roadmap/referred_by">
        <owl:inverseOf rdf:resource="http://ontology.decidim.org/decidim_roadmap/refers_to"/>
        <rdfs:range rdf:resource="http://ontology.decidim.org/decidim_roadmap/ParticipationItem"/>
        <rdfs:comment xml:lang="en">This general property indicates that an entity points to an Item that refers to it in some way. This may be because the entity is mentioned, references, amended or replied to by the Item. Specific subproperties help distinguish these different cases.

It is inverse property of refers_to.</rdfs:comment>
        <rdfs:label xml:lang="en">referred by</rdfs:label>
    </owl:ObjectProperty>
    


    <!-- http://ontology.decidim.org/decidim_roadmap/refers_to -->

    <owl:ObjectProperty rdf:about="http://ontology.decidim.org/decidim_roadmap/refers_to">
        <rdfs:domain rdf:resource="http://ontology.decidim.org/decidim_roadmap/ParticipationItem"/>
        <rdfs:comment xml:lang="en">This general property indicates that an Item points to an entity is referred to in some way. This may be because the Item mentions, references, amends or replies to it. Specific subproperties help distinguish these different cases.

It is inverse property of referred_by.</rdfs:comment>
        <rdfs:label xml:lang="en">refers to</rdfs:label>
    </owl:ObjectProperty>
    


    <!-- http://ontology.decidim.org/decidim_roadmap/related_to -->

    <owl:ObjectProperty rdf:about="http://ontology.decidim.org/decidim_roadmap/related_to">
        <rdf:type rdf:resource="http://www.w3.org/2002/07/owl#SymmetricProperty"/>
        <rdfs:comment xml:lang="en">Symmetric object property indicating that two individual are related to each other.</rdfs:comment>
    </owl:ObjectProperty>
    


    <!-- http://ontology.decidim.org/decidim_roadmap/reply_of -->

    <owl:ObjectProperty rdf:about="http://ontology.decidim.org/decidim_roadmap/reply_of">
        <rdfs:subPropertyOf rdf:resource="http://ontology.decidim.org/decidim_roadmap/refers_to"/>
        <rdf:type rdf:resource="http://www.w3.org/2002/07/owl#FunctionalProperty"/>
        <rdfs:domain rdf:resource="http://ontology.decidim.org/decidim_roadmap/Comment"/>
        <rdfs:range rdf:resource="http://ontology.decidim.org/decidim_roadmap/ParticipationItem"/>
        <rdfs:comment xml:lang="en">Points to an Item which this Comment replies to.</rdfs:comment>
        <rdfs:label xml:lang="en">reply of</rdfs:label>
    </owl:ObjectProperty>
    


    <!-- http://ontology.decidim.org/decidim_roadmap/reported_by -->

    <owl:ObjectProperty rdf:about="http://ontology.decidim.org/decidim_roadmap/reported_by">
        <rdfs:subPropertyOf rdf:resource="http://ontology.decidim.org/decidim_roadmap/has_actor"/>
        <owl:inverseOf rdf:resource="http://ontology.decidim.org/decidim_roadmap/reports"/>
        <rdfs:domain rdf:resource="http://ontology.decidim.org/decidim_roadmap/ParticipationItem"/>
        <rdfs:range rdf:resource="http://ontology.decidim.org/decidim_roadmap/#RegisteredParticipant"/>
        <rdfs:label xml:lang="en">reported by</rdfs:label>
    </owl:ObjectProperty>
    


    <!-- http://ontology.decidim.org/decidim_roadmap/reports -->

    <owl:ObjectProperty rdf:about="http://ontology.decidim.org/decidim_roadmap/reports">
        <rdfs:subPropertyOf rdf:resource="http://ontology.decidim.org/decidim_roadmap/acts_on"/>
        <rdfs:domain rdf:resource="http://ontology.decidim.org/decidim_roadmap/#RegisteredParticipant"/>
        <rdfs:range rdf:resource="http://ontology.decidim.org/decidim_roadmap/ParticipationItem"/>
        <rdfs:label xml:lang="en">reports</rdfs:label>
    </owl:ObjectProperty>
    


    <!-- http://ontology.decidim.org/decidim_roadmap/result_of -->

    <owl:ObjectProperty rdf:about="http://ontology.decidim.org/decidim_roadmap/result_of">
        <rdfs:subPropertyOf rdf:resource="http://ontology.decidim.org/decidim_roadmap/refers_to"/>
        <rdfs:domain rdf:resource="http://ontology.decidim.org/decidim_roadmap/Result"/>
        <rdfs:range rdf:resource="http://ontology.decidim.org/decidim_roadmap/Proposal"/>
        <rdfs:label>result of</rdfs:label>
    </owl:ObjectProperty>
    


    <!-- http://ontology.decidim.org/decidim_roadmap/role_of -->

    <owl:ObjectProperty rdf:about="http://ontology.decidim.org/decidim_roadmap/role_of">
        <rdfs:subPropertyOf rdf:resource="http://ontology.decidim.org/decidim_roadmap/specifies"/>
        <rdfs:domain rdf:resource="http://ontology.decidim.org/decidim_roadmap/Role"/>
        <rdfs:range rdf:resource="http://ontology.decidim.org/decidim_roadmap/#RegisteredParticipant"/>
        <rdfs:label>role of</rdfs:label>
    </owl:ObjectProperty>
    


    <!-- http://ontology.decidim.org/decidim_roadmap/role_scope_of -->

    <owl:ObjectProperty rdf:about="http://ontology.decidim.org/decidim_roadmap/role_scope_of">
        <rdfs:subPropertyOf rdf:resource="http://ontology.decidim.org/decidim_roadmap/specifies"/>
        <rdfs:domain rdf:resource="http://ontology.decidim.org/decidim_roadmap/ParticipationArtifact"/>
        <rdfs:range rdf:resource="http://ontology.decidim.org/decidim_roadmap/Role"/>
        <rdfs:label>role scope of</rdfs:label>
    </owl:ObjectProperty>
    


    <!-- http://ontology.decidim.org/decidim_roadmap/scope_of -->

    <owl:ObjectProperty rdf:about="http://ontology.decidim.org/decidim_roadmap/scope_of">
        <rdfs:subPropertyOf rdf:resource="http://ontology.decidim.org/decidim_roadmap/specifies"/>
        <rdfs:label>scope of</rdfs:label>
    </owl:ObjectProperty>
    


    <!-- http://ontology.decidim.org/decidim_roadmap/similar_to -->

    <owl:ObjectProperty rdf:about="http://ontology.decidim.org/decidim_roadmap/similar_to">
        <rdfs:subPropertyOf rdf:resource="http://ontology.decidim.org/decidim_roadmap/related_to"/>
        <rdfs:domain rdf:resource="http://ontology.decidim.org/decidim_roadmap/ParticipationItem"/>
        <rdfs:range rdf:resource="http://ontology.decidim.org/decidim_roadmap/ParticipationItem"/>
        <rdfs:comment xml:lang="en">Symmetric object property that indicates that two Participation items (e.g., two Proposals) are similar to each other.</rdfs:comment>
    </owl:ObjectProperty>
    


    <!-- http://ontology.decidim.org/decidim_roadmap/specified_by -->

    <owl:ObjectProperty rdf:about="http://ontology.decidim.org/decidim_roadmap/specified_by">
        <owl:inverseOf rdf:resource="http://ontology.decidim.org/decidim_roadmap/specifies"/>
        <rdfs:comment xml:lang="en">General property that indicates that some aspect or attribute of the entity is specified by an other one.</rdfs:comment>
        <rdfs:label xml:lang="en">specified by</rdfs:label>
    </owl:ObjectProperty>
    


    <!-- http://ontology.decidim.org/decidim_roadmap/specifies -->

    <owl:ObjectProperty rdf:about="http://ontology.decidim.org/decidim_roadmap/specifies">
        <rdfs:comment xml:lang="en">General property that indicates that an entity specifies an aspect or attribute of another entity, such as its Scope, Category or Role.

It is inverse property of specified_by.</rdfs:comment>
        <rdfs:label xml:lang="en">specifies</rdfs:label>
    </owl:ObjectProperty>
    


    <!-- http://ontology.decidim.org/decidim_roadmap/subcategory_of -->

    <owl:ObjectProperty rdf:about="http://ontology.decidim.org/decidim_roadmap/subcategory_of">
        <rdfs:subPropertyOf rdf:resource="http://ontology.decidim.org/decidim_roadmap/belong_to"/>
        <rdfs:domain rdf:resource="http://ontology.decidim.org/decidim_roadmap/Category"/>
        <rdfs:range rdf:resource="http://ontology.decidim.org/decidim_roadmap/Category"/>
        <rdfs:label xml:lang="en">subcategory of</rdfs:label>
    </owl:ObjectProperty>
    


    <!-- http://ontology.decidim.org/decidim_roadmap/subgroup_of -->

    <owl:ObjectProperty rdf:about="http://ontology.decidim.org/decidim_roadmap/subgroup_of">
        <rdfs:subPropertyOf rdf:resource="http://ontology.decidim.org/decidim_roadmap/belong_to"/>
        <rdfs:domain rdf:resource="http://ontology.decidim.org/decidim_roadmap/Group"/>
        <rdfs:range rdf:resource="http://ontology.decidim.org/decidim_roadmap/Group"/>
        <rdfs:label xml:lang="en">subgroup of</rdfs:label>
    </owl:ObjectProperty>
    


    <!-- http://ontology.decidim.org/decidim_roadmap/supporter_of -->

    <owl:ObjectProperty rdf:about="http://ontology.decidim.org/decidim_roadmap/supporter_of">
        <rdfs:subPropertyOf rdf:resource="http://ontology.decidim.org/decidim_roadmap/acts_on"/>
        <rdfs:domain rdf:resource="http://ontology.decidim.org/decidim_roadmap/VerifiedPerson"/>
        <rdfs:range rdf:resource="http://ontology.decidim.org/decidim_roadmap/Proposal"/>
        <rdfs:label xml:lang="en">supporter of</rdfs:label>
        <rdfs:label>supports</rdfs:label>
    </owl:ObjectProperty>
    


    <!-- http://ontology.decidim.org/decidim_roadmap/votes_comment -->

    <owl:ObjectProperty rdf:about="http://ontology.decidim.org/decidim_roadmap/votes_comment">
        <rdfs:subPropertyOf rdf:resource="http://ontology.decidim.org/decidim_roadmap/acts_on"/>
        <rdfs:domain rdf:resource="http://ontology.decidim.org/decidim_roadmap/#RegisteredParticipant"/>
        <rdfs:range rdf:resource="http://ontology.decidim.org/decidim_roadmap/Comment"/>
        <rdfs:label>votes comment</rdfs:label>
    </owl:ObjectProperty>
    


    <!-- http://ontology.decidim.org/decidim_roadmap/withdrawn_by -->

    <owl:ObjectProperty rdf:about="http://ontology.decidim.org/decidim_roadmap/withdrawn_by">
        <rdfs:subPropertyOf rdf:resource="http://ontology.decidim.org/decidim_roadmap/has_actor"/>
        <owl:inverseOf rdf:resource="http://ontology.decidim.org/decidim_roadmap/withdraws"/>
        <rdfs:domain rdf:resource="http://ontology.decidim.org/decidim_roadmap/#RegisteredParticipant"/>
        <rdfs:range rdf:resource="http://ontology.decidim.org/decidim_roadmap/Proposal"/>
        <rdfs:label xml:lang="en">withdrawn by</rdfs:label>
    </owl:ObjectProperty>
    


    <!-- http://ontology.decidim.org/decidim_roadmap/withdraws -->

    <owl:ObjectProperty rdf:about="http://ontology.decidim.org/decidim_roadmap/withdraws">
        <rdfs:subPropertyOf rdf:resource="http://ontology.decidim.org/decidim_roadmap/acts_on"/>
        <rdfs:domain rdf:resource="http://ontology.decidim.org/decidim_roadmap/#RegisteredParticipant"/>
        <rdfs:range rdf:resource="http://ontology.decidim.org/decidim_roadmap/Proposal"/>
        <rdfs:label xml:lang="en">withdraws</rdfs:label>
    </owl:ObjectProperty>
    


    <!-- 
    ///////////////////////////////////////////////////////////////////////////////////////
    //
    // Classes
    //
    ///////////////////////////////////////////////////////////////////////////////////////
     -->

    


    <!-- http://ontology.decidim.org/decidim_roadmap/AccountabilityContainer -->

    <owl:Class rdf:about="http://ontology.decidim.org/decidim_roadmap/AccountabilityContainer">
        <rdfs:subClassOf rdf:resource="http://ontology.decidim.org/decidim_roadmap/Container"/>
        <rdfs:subClassOf>
            <owl:Restriction>
                <owl:onProperty rdf:resource="http://ontology.decidim.org/decidim_roadmap/container_of"/>
                <owl:someValuesFrom rdf:resource="http://ontology.decidim.org/decidim_roadmap/Result"/>
            </owl:Restriction>
        </rdfs:subClassOf>
        <rdfs:comment xml:lang="en">This functionality allows participants to monitor the results of a participation space, and the progress of derived projects.

It is a ParticipationFunctionality of kind Container, and includes Items of kind Result, vinculated to the corresponding accepted Proposals and to projects deriving from them.</rdfs:comment>
        <rdfs:label xml:lang="en">Accountability container</rdfs:label>
    </owl:Class>
    


    <!-- http://ontology.decidim.org/decidim_roadmap/Administrator -->

    <owl:Class rdf:about="http://ontology.decidim.org/decidim_roadmap/Administrator">
        <rdfs:subClassOf rdf:resource="http://ontology.decidim.org/decidim_roadmap/Moderator"/>
        <rdfs:comment xml:lang="en">A registered participant who has the role of Administrator on a ParticipationArtifact can configure and manage it, and can grant other RegisteredParticipants administration permissions of Collaborator, Moderator or Administrator in the same ParticipationArtifact or on a ParticipationArtifact contained in it.</rdfs:comment>
        <rdfs:label xml:lang="en">Administrator</rdfs:label>
    </owl:Class>
    


    <!-- http://ontology.decidim.org/decidim_roadmap/Amendment -->

    <owl:Class rdf:about="http://ontology.decidim.org/decidim_roadmap/Amendment">
        <rdfs:subClassOf rdf:resource="http://ontology.decidim.org/decidim_roadmap/Proposal"/>
        <rdfs:subClassOf>
            <owl:Restriction>
                <owl:onProperty rdf:resource="http://ontology.decidim.org/decidim_roadmap/amendment_of"/>
                <owl:qualifiedCardinality rdf:datatype="http://www.w3.org/2001/XMLSchema#nonNegativeInteger">1</owl:qualifiedCardinality>
                <owl:onClass rdf:resource="http://ontology.decidim.org/decidim_roadmap/Proposal"/>
            </owl:Restriction>
        </rdfs:subClassOf>
        <rdfs:comment xml:lang="en">An Amendment is a kind of Proposal that refers to a specific Proposal it proposes to enmend, to which it is linked through the property amendment_of.</rdfs:comment>
        <rdfs:label xml:lang="en">Amendment</rdfs:label>
    </owl:Class>
    


    <!-- http://ontology.decidim.org/decidim_roadmap/Assembly -->

    <owl:Class rdf:about="http://ontology.decidim.org/decidim_roadmap/Assembly">
        <rdfs:subClassOf rdf:resource="http://ontology.decidim.org/decidim_roadmap/Group"/>
        <rdfs:subClassOf rdf:resource="http://ontology.decidim.org/decidim_roadmap/#ParticipationSpace"/>
        <rdfs:subClassOf>
            <owl:Restriction>
                <owl:onProperty rdf:resource="http://ontology.decidim.org/decidim_roadmap/has_promoter"/>
                <owl:someValuesFrom rdf:resource="http://ontology.decidim.org/decidim_roadmap/SovereignOrganization"/>
            </owl:Restriction>
        </rdfs:subClassOf>
        <owl:disjointWith rdf:resource="http://ontology.decidim.org/decidim_roadmap/Consultation"/>
        <owl:disjointWith rdf:resource="http://ontology.decidim.org/decidim_roadmap/Initiative"/>
        <owl:disjointWith rdf:resource="http://ontology.decidim.org/decidim_roadmap/Process"/>
        <owl:disjointWith rdf:resource="http://ontology.decidim.org/decidim_roadmap/ProcessGroup"/>
        <rdfs:comment xml:lang="en">An assembly is a participation space, defined as a structured group of participants that meet periodically, individually or representatively, and can create proposals and make decisions. Beyond being a Participation space, an assembly is also a Group, and as such it can be the promoter of a Process, or participate in other participation spaces.

An Assembly may have WorkingGroups, i.e. subgroups created to work on specific issues.</rdfs:comment>
        <rdfs:label xml:lang="en">Assembly</rdfs:label>
    </owl:Class>
    


    <!-- http://ontology.decidim.org/decidim_roadmap/Attribute -->

    <owl:Class rdf:about="http://ontology.decidim.org/decidim_roadmap/Attribute">
        <rdfs:comment xml:lang="en">General class for entities that represent an attribute of other entities, such as their Scope or Category.</rdfs:comment>
        <rdfs:label xml:lang="en">Attribute</rdfs:label>
    </owl:Class>
    


    <!-- http://ontology.decidim.org/decidim_roadmap/AuthoredItem -->

    <owl:Class rdf:about="http://ontology.decidim.org/decidim_roadmap/AuthoredItem">
        <rdfs:subClassOf rdf:resource="http://ontology.decidim.org/decidim_roadmap/ParticipationItem"/>
        <rdfs:subClassOf>
            <owl:Restriction>
                <owl:onProperty rdf:resource="http://ontology.decidim.org/decidim_roadmap/has_creator"/>
                <owl:someValuesFrom rdf:resource="http://ontology.decidim.org/decidim_roadmap/#RegisteredParticipant"/>
            </owl:Restriction>
        </rdfs:subClassOf>
        <rdfs:comment xml:lang="en">This class represents Items that have an author. While some content in the Platform and ParticipationSpaces is created by the Adinistrators, AuthoredItems have a creator that can typically be any RegisteredParticipant.</rdfs:comment>
        <rdfs:label xml:lang="en">Authored resource</rdfs:label>
    </owl:Class>
    


    <!-- http://ontology.decidim.org/decidim_roadmap/Blog -->

    <owl:Class rdf:about="http://ontology.decidim.org/decidim_roadmap/Blog">
        <rdfs:subClassOf rdf:resource="http://ontology.decidim.org/decidim_roadmap/Container"/>
        <rdfs:subClassOf>
            <owl:Restriction>
                <owl:onProperty rdf:resource="http://ontology.decidim.org/decidim_roadmap/container_of"/>
                <owl:someValuesFrom rdf:resource="http://ontology.decidim.org/decidim_roadmap/Blog_post"/>
            </owl:Restriction>
        </rdfs:subClassOf>
        <rdfs:subClassOf>
            <owl:Restriction>
                <owl:onProperty rdf:resource="http://ontology.decidim.org/decidim_roadmap/container_of"/>
                <owl:someValuesFrom rdf:resource="http://ontology.decidim.org/decidim_roadmap/Thread"/>
            </owl:Restriction>
        </rdfs:subClassOf>
        <rdfs:comment xml:lang="en">A Blog allows for the reation of pieces of content (BlogPosts) in shown in chronological order and classified according to the patform&apos;s content categorization system.

A Blog is a ParticipationFunctionality of kind Container, that includes Items of kind BlogPost. Blog posts can in turn receive comments and conversation Threads, analogously to Proposals and other Items.</rdfs:comment>
        <rdfs:label xml:lang="en">Blog</rdfs:label>
    </owl:Class>
    


    <!-- http://ontology.decidim.org/decidim_roadmap/Blog_post -->

    <owl:Class rdf:about="http://ontology.decidim.org/decidim_roadmap/Blog_post">
        <rdfs:subClassOf rdf:resource="http://ontology.decidim.org/decidim_roadmap/ParticipationItem"/>
        <rdfs:subClassOf>
            <owl:Restriction>
                <owl:onProperty rdf:resource="http://ontology.decidim.org/decidim_roadmap/has_container"/>
                <owl:qualifiedCardinality rdf:datatype="http://www.w3.org/2001/XMLSchema#nonNegativeInteger">1</owl:qualifiedCardinality>
                <owl:onClass rdf:resource="http://ontology.decidim.org/decidim_roadmap/Blog"/>
            </owl:Restriction>
        </rdfs:subClassOf>
        <rdfs:comment xml:lang="en">A BlogPost is a piece of content that is published within a Blog.</rdfs:comment>
        <rdfs:label xml:lang="en">Blog post</rdfs:label>
    </owl:Class>
    


    <!-- http://ontology.decidim.org/decidim_roadmap/BudgetedProject -->

    <owl:Class rdf:about="http://ontology.decidim.org/decidim_roadmap/BudgetedProject">
        <rdfs:subClassOf rdf:resource="http://ontology.decidim.org/decidim_roadmap/AuthoredItem"/>
        <rdfs:subClassOf>
            <owl:Restriction>
                <owl:onProperty rdf:resource="http://ontology.decidim.org/decidim_roadmap/has_container"/>
                <owl:qualifiedCardinality rdf:datatype="http://www.w3.org/2001/XMLSchema#nonNegativeInteger">1</owl:qualifiedCardinality>
                <owl:onClass rdf:resource="http://ontology.decidim.org/decidim_roadmap/ParticipativeBudget"/>
            </owl:Restriction>
        </rdfs:subClassOf>
        <rdfs:subClassOf>
            <owl:Restriction>
                <owl:onProperty rdf:resource="http://ontology.decidim.org/decidim_roadmap/has_creator"/>
                <owl:qualifiedCardinality rdf:datatype="http://www.w3.org/2001/XMLSchema#nonNegativeInteger">1</owl:qualifiedCardinality>
                <owl:onClass rdf:resource="http://ontology.decidim.org/decidim_roadmap/#RegisteredParticipant"/>
            </owl:Restriction>
        </rdfs:subClassOf>
        <rdfs:comment xml:lang="en">A kind of proposal, that has a budget associated with it.</rdfs:comment>
        <rdfs:label xml:lang="en">Budgeted project</rdfs:label>
    </owl:Class>
    


    <!-- http://ontology.decidim.org/decidim_roadmap/Category -->

    <owl:Class rdf:about="http://ontology.decidim.org/decidim_roadmap/Category">
        <rdfs:subClassOf rdf:resource="http://ontology.decidim.org/decidim_roadmap/Attribute"/>
        <rdfs:comment xml:lang="en">Categories are used to group items according to some criteria, typically the topic. They help participants browse and search information in a Participation space.</rdfs:comment>
        <rdfs:label xml:lang="en">Category</rdfs:label>
    </owl:Class>
    


    <!-- http://ontology.decidim.org/decidim_roadmap/Collaborator -->

    <owl:Class rdf:about="http://ontology.decidim.org/decidim_roadmap/Collaborator">
        <rdfs:subClassOf rdf:resource="http://ontology.decidim.org/decidim_roadmap/Role"/>
        <rdfs:comment xml:lang="en">A RegisteredParticipant having the Role of Collaborator in a given role scope can access the same information as an Administrator, including configuration panels, but cannot modify it.</rdfs:comment>
        <rdfs:label xml:lang="en">Collaborator</rdfs:label>
    </owl:Class>
    


    <!-- http://ontology.decidim.org/decidim_roadmap/Comment -->

    <owl:Class rdf:about="http://ontology.decidim.org/decidim_roadmap/Comment">
        <rdfs:subClassOf rdf:resource="http://ontology.decidim.org/decidim_roadmap/AuthoredItem"/>
        <rdfs:subClassOf>
            <owl:Restriction>
                <owl:onProperty rdf:resource="http://ontology.decidim.org/decidim_roadmap/has_creator"/>
                <owl:qualifiedCardinality rdf:datatype="http://www.w3.org/2001/XMLSchema#nonNegativeInteger">1</owl:qualifiedCardinality>
                <owl:onClass rdf:resource="http://ontology.decidim.org/decidim_roadmap/#RegisteredParticipant"/>
            </owl:Restriction>
        </rdfs:subClassOf>
        <rdfs:subClassOf>
            <owl:Restriction>
                <owl:onProperty rdf:resource="http://ontology.decidim.org/decidim_roadmap/reply_of"/>
                <owl:qualifiedCardinality rdf:datatype="http://www.w3.org/2001/XMLSchema#nonNegativeInteger">1</owl:qualifiedCardinality>
                <owl:onClass rdf:resource="http://ontology.decidim.org/decidim_roadmap/ParticipationItem"/>
            </owl:Restriction>
        </rdfs:subClassOf>
        <rdfs:comment xml:lang="en">Comments are ParticipationItems authored by RegisteredParticipants, that can be associated with different ParticipationFunctionalities and Items. 

A Comment can be referred to another comment (NestedComment) or to some other ParticipationItem (FirstLevelComment).</rdfs:comment>
        <rdfs:label xml:lang="en">Comment</rdfs:label>
    </owl:Class>
    


    <!-- http://ontology.decidim.org/decidim_roadmap/Configurator -->

    <owl:Class rdf:about="http://ontology.decidim.org/decidim_roadmap/Configurator">
        <rdfs:subClassOf rdf:resource="http://ontology.decidim.org/decidim_roadmap/ParticipationArtifact"/>
        <rdfs:subClassOf>
            <owl:Restriction>
                <owl:onProperty rdf:resource="http://ontology.decidim.org/decidim_roadmap/configurator_of"/>
                <owl:qualifiedCardinality rdf:datatype="http://www.w3.org/2001/XMLSchema#nonNegativeInteger">1</owl:qualifiedCardinality>
                <owl:onClass rdf:resource="http://ontology.decidim.org/decidim_roadmap/ParticipationArtifact"/>
            </owl:Restriction>
        </rdfs:subClassOf>
        <rdfs:comment xml:lang="en">Administration panel associated to a ParticipationArtifact, that allows Administrators to configure it. Collaborators of the artifat can access the configurator but not modify it; moderators can also access the configurator, and additionally they can manage certain aspects such as accepting or rejecting proposals.
A Configurator is linked to the ParticipationArtifacts it allows to configure through the property configurator_of.</rdfs:comment>
        <rdfs:label xml:lang="en">Configurator</rdfs:label>
    </owl:Class>
    


    <!-- http://ontology.decidim.org/decidim_roadmap/Consultation -->

    <owl:Class rdf:about="http://ontology.decidim.org/decidim_roadmap/Consultation">
        <rdfs:subClassOf rdf:resource="http://ontology.decidim.org/decidim_roadmap/#ParticipationSpace"/>
        <rdfs:subClassOf>
            <owl:Restriction>
                <owl:onProperty rdf:resource="http://ontology.decidim.org/decidim_roadmap/has_promoter"/>
                <owl:someValuesFrom rdf:resource="http://ontology.decidim.org/decidim_roadmap/SovereignOrganization"/>
            </owl:Restriction>
        </rdfs:subClassOf>
        <owl:disjointWith rdf:resource="http://ontology.decidim.org/decidim_roadmap/Initiative"/>
        <owl:disjointWith rdf:resource="http://ontology.decidim.org/decidim_roadmap/Process"/>
        <owl:disjointWith rdf:resource="http://ontology.decidim.org/decidim_roadmap/ProcessGroup"/>
        <rdfs:comment xml:lang="en">A Consultation is a ParticipationSpace that allows a votation on some issue, involving all the participants of the SovereignOrganization promoting it. Participants can not only vote, but also get information, debate and monitor the results.</rdfs:comment>
        <rdfs:label xml:lang="en">Consultation</rdfs:label>
    </owl:Class>
    


    <!-- http://ontology.decidim.org/decidim_roadmap/Container -->

    <owl:Class rdf:about="http://ontology.decidim.org/decidim_roadmap/Container">
        <rdfs:subClassOf rdf:resource="http://ontology.decidim.org/decidim_roadmap/ParticipationFunctionality"/>
        <rdfs:comment xml:lang="en">Functionalities of this kind contain ParticipationItems, to which they are linked to the property container_of. 

Different kinds of ParticipationContainers contain different kinds of ParticipationItems: for example, a Debate contains items of ind Thread and Comment, a ProposalIncubator contains Proposals, a ParticipativeBudget contains BudgetedProposals and a MeetingCalendar contains Meetings.</rdfs:comment>
        <rdfs:label xml:lang="en">Container</rdfs:label>
    </owl:Class>
    


    <!-- http://ontology.decidim.org/decidim_roadmap/Debate -->

    <owl:Class rdf:about="http://ontology.decidim.org/decidim_roadmap/Debate">
        <rdfs:subClassOf rdf:resource="http://ontology.decidim.org/decidim_roadmap/Container"/>
        <rdfs:subClassOf>
            <owl:Restriction>
                <owl:onProperty rdf:resource="http://ontology.decidim.org/decidim_roadmap/container_of"/>
                <owl:someValuesFrom rdf:resource="http://ontology.decidim.org/decidim_roadmap/Blog_post"/>
            </owl:Restriction>
        </rdfs:subClassOf>
        <rdfs:subClassOf>
            <owl:Restriction>
                <owl:onProperty rdf:resource="http://ontology.decidim.org/decidim_roadmap/container_of"/>
                <owl:someValuesFrom rdf:resource="http://ontology.decidim.org/decidim_roadmap/Thread"/>
            </owl:Restriction>
        </rdfs:subClassOf>
        <rdfs:comment xml:lang="en">This functionality allows for the creation of debates about specific questions, defined by the Administrators or by RegisteredParticipants.

A Debate is a ParticipationFunctionality of kind Container, that includes Items of kind Comment, and the corresponding Threads.</rdfs:comment>
        <rdfs:label xml:lang="en">Debate</rdfs:label>
    </owl:Class>
    


    <!-- http://ontology.decidim.org/decidim_roadmap/FirstLevelComment -->

    <owl:Class rdf:about="http://ontology.decidim.org/decidim_roadmap/FirstLevelComment">
        <rdfs:subClassOf rdf:resource="http://ontology.decidim.org/decidim_roadmap/Comment"/>
        <owl:disjointWith rdf:resource="http://ontology.decidim.org/decidim_roadmap/NestedComment"/>
        <rdfs:comment xml:lang="en">A comment referred to some ParticipationItem, which is not another comment.</rdfs:comment>
        <rdfs:label xml:lang="en">First level comment</rdfs:label>
    </owl:Class>
    


    <!-- http://ontology.decidim.org/decidim_roadmap/Group -->

    <owl:Class rdf:about="http://ontology.decidim.org/decidim_roadmap/Group">
        <rdfs:subClassOf rdf:resource="http://ontology.decidim.org/decidim_roadmap/Organization"/>
        <rdfs:subClassOf>
            <owl:Restriction>
                <owl:onProperty rdf:resource="http://ontology.decidim.org/decidim_roadmap/has_member"/>
                <owl:someValuesFrom rdf:resource="http://ontology.decidim.org/decidim_roadmap/#RegisteredParticipant"/>
            </owl:Restriction>
        </rdfs:subClassOf>
        <owl:disjointWith rdf:resource="http://ontology.decidim.org/decidim_roadmap/RegisteredPerson"/>
        <rdfs:comment xml:lang="en">A collective account corresponding to a group of registered participants.</rdfs:comment>
        <rdfs:label xml:lang="en">Group</rdfs:label>
    </owl:Class>
    


    <!-- http://ontology.decidim.org/decidim_roadmap/Initiative -->

    <owl:Class rdf:about="http://ontology.decidim.org/decidim_roadmap/Initiative">
        <rdfs:subClassOf rdf:resource="http://ontology.decidim.org/decidim_roadmap/#ParticipationSpace"/>
        <rdfs:subClassOf>
            <owl:Restriction>
                <owl:onProperty rdf:resource="http://ontology.decidim.org/decidim_roadmap/has_promoter"/>
                <owl:someValuesFrom rdf:resource="http://ontology.decidim.org/decidim_roadmap/#VerifiedParticipant"/>
            </owl:Restriction>
        </rdfs:subClassOf>
        <rdfs:subClassOf>
            <owl:Restriction>
                <owl:onProperty rdf:resource="http://ontology.decidim.org/decidim_roadmap/initiative_of"/>
                <owl:qualifiedCardinality rdf:datatype="http://www.w3.org/2001/XMLSchema#nonNegativeInteger">1</owl:qualifiedCardinality>
                <owl:onClass rdf:resource="http://ontology.decidim.org/decidim_roadmap/Proposal"/>
            </owl:Restriction>
        </rdfs:subClassOf>
        <owl:disjointWith rdf:resource="http://ontology.decidim.org/decidim_roadmap/Process"/>
        <owl:disjointWith rdf:resource="http://ontology.decidim.org/decidim_roadmap/ProcessGroup"/>
        <rdfs:comment xml:lang="en">While a Process is necessarily promoted by an organization, an Initiative is a ParticipationSpace that can be promoted by any VerifiedParticipant, i.e. by any individual citizen or organization whose account has been verified to correspond to their real identity. 

An Initiative is always connected to a Proposal it promotes, with the goal of gathering support for it, and to be considered for acceptance by the SovereignOrganization running the ParticipationPlatform.</rdfs:comment>
        <rdfs:label xml:lang="en">Initiative</rdfs:label>
    </owl:Class>
    


    <!-- http://ontology.decidim.org/decidim_roadmap/ManagedAccount -->

    <owl:Class rdf:about="http://ontology.decidim.org/decidim_roadmap/ManagedAccount">
        <rdfs:subClassOf rdf:resource="http://ontology.decidim.org/decidim_roadmap/VerifiedPerson"/>
        <rdfs:comment xml:lang="en">A ManagedAccount is an account managed on behalf of another Person, that for some reason is not able to manage it by themselves.</rdfs:comment>
        <rdfs:label xml:lang="en">Managed account</rdfs:label>
    </owl:Class>
    


    <!-- http://ontology.decidim.org/decidim_roadmap/Meeting -->

    <owl:Class rdf:about="http://ontology.decidim.org/decidim_roadmap/Meeting">
        <rdfs:subClassOf rdf:resource="http://ontology.decidim.org/decidim_roadmap/ParticipationItem"/>
        <rdfs:subClassOf>
            <owl:Restriction>
                <owl:onProperty rdf:resource="http://ontology.decidim.org/decidim_roadmap/has_attendee"/>
                <owl:someValuesFrom rdf:resource="http://ontology.decidim.org/decidim_roadmap/#RegisteredParticipant"/>
            </owl:Restriction>
        </rdfs:subClassOf>
        <rdfs:comment xml:lang="en">A Meeting is a physical gathering in which RegisteredParticipants can meet presentially to discuss about some issue and create Proposals. 

A Meeting is linked to the participants attending it through the property has_attendee.

A Meeting can be included in a Workshop or in an EventCalendar associated to some ParticipationSpace.</rdfs:comment>
        <rdfs:label xml:lang="en">Meeting</rdfs:label>
    </owl:Class>
    


    <!-- http://ontology.decidim.org/decidim_roadmap/MeetingCalendar -->

    <owl:Class rdf:about="http://ontology.decidim.org/decidim_roadmap/MeetingCalendar">
        <rdfs:subClassOf rdf:resource="http://ontology.decidim.org/decidim_roadmap/Container"/>
        <rdfs:subClassOf>
            <owl:Restriction>
                <owl:onProperty rdf:resource="http://ontology.decidim.org/decidim_roadmap/container_of"/>
                <owl:someValuesFrom rdf:resource="http://ontology.decidim.org/decidim_roadmap/Meeting"/>
            </owl:Restriction>
        </rdfs:subClassOf>
        <rdfs:comment xml:lang="en">A MeetingCalendar is a group of meetings associated to a given ParticipationSpace. 

Like a Workshop, it is a ParticipationFunctionality of kind Container, that includes Item of kind Meeting; however, in this case events may typically span over a long period of time, be located in different places and not be related to each other.</rdfs:comment>
        <rdfs:label xml:lang="en">Meeting calendar</rdfs:label>
    </owl:Class>
    


    <!-- http://ontology.decidim.org/decidim_roadmap/Moderator -->

    <owl:Class rdf:about="http://ontology.decidim.org/decidim_roadmap/Moderator">
        <rdfs:subClassOf rdf:resource="http://ontology.decidim.org/decidim_roadmap/Collaborator"/>
        <rdfs:comment xml:lang="en">The role of Moderator attributes to a RegisteredParticipant the same rights as a Collaborator for accessing information, plus the possibility of managing ParticipationArtifacts within the role&apos;s scope (for example, they can assign a status to a Proposal, and provide an official response).</rdfs:comment>
        <rdfs:label xml:lang="en">Moderator</rdfs:label>
    </owl:Class>
    


    <!-- http://ontology.decidim.org/decidim_roadmap/NestedComment -->

    <owl:Class rdf:about="http://ontology.decidim.org/decidim_roadmap/NestedComment">
        <rdfs:subClassOf rdf:resource="http://ontology.decidim.org/decidim_roadmap/Comment"/>
        <rdfs:subClassOf>
            <owl:Restriction>
                <owl:onProperty rdf:resource="http://ontology.decidim.org/decidim_roadmap/reply_of"/>
                <owl:qualifiedCardinality rdf:datatype="http://www.w3.org/2001/XMLSchema#nonNegativeInteger">1</owl:qualifiedCardinality>
                <owl:onClass rdf:resource="http://ontology.decidim.org/decidim_roadmap/Comment"/>
            </owl:Restriction>
        </rdfs:subClassOf>
        <rdfs:comment xml:lang="en">A comment that replies to another comment.</rdfs:comment>
        <rdfs:label xml:lang="en">Nested comment</rdfs:label>
    </owl:Class>
    


    <!-- http://ontology.decidim.org/decidim_roadmap/Newsletter -->

    <owl:Class rdf:about="http://ontology.decidim.org/decidim_roadmap/Newsletter">
        <rdfs:subClassOf rdf:resource="http://ontology.decidim.org/decidim_roadmap/ParticipationFunctionality"/>
        <rdfs:comment xml:lang="en">A Newsletter allows to broadcast messages to all the RegisteredParticipants associated to a ParticipationPlatform or to a specific ParticipationSpace.</rdfs:comment>
        <rdfs:label xml:lang="en">Newsletter</rdfs:label>
    </owl:Class>
    


    <!-- http://ontology.decidim.org/decidim_roadmap/OfficialAccount -->

    <owl:Class rdf:about="http://ontology.decidim.org/decidim_roadmap/OfficialAccount">
        <rdfs:subClassOf rdf:resource="http://ontology.decidim.org/decidim_roadmap/VerifiedPerson"/>
        <rdfs:comment xml:lang="en">A verified person whose account name has also been verified to correspond to the real name.</rdfs:comment>
        <rdfs:label>Official account</rdfs:label>
    </owl:Class>
    


    <!-- http://ontology.decidim.org/decidim_roadmap/Organization -->

    <owl:Class rdf:about="http://ontology.decidim.org/decidim_roadmap/Organization">
        <rdfs:subClassOf rdf:resource="http://ontology.decidim.org/decidim_roadmap/#Agent"/>
        <owl:disjointWith rdf:resource="http://ontology.decidim.org/decidim_roadmap/Person"/>
        <rdfs:comment xml:lang="en">An organized group of people with a collective purpose. Specific subclasses represent the case of groups of registered participants (Group), and the organization promoting a ParticipationPlatform or a ParticipationSpace (Sovereign organization).</rdfs:comment>
        <rdfs:label xml:lang="en">Organization</rdfs:label>
    </owl:Class>
    


    <!-- http://ontology.decidim.org/decidim_roadmap/Page -->

    <owl:Class rdf:about="http://ontology.decidim.org/decidim_roadmap/Page">
        <rdfs:subClassOf rdf:resource="http://ontology.decidim.org/decidim_roadmap/ParticipationFunctionality"/>
        <rdfs:comment xml:lang="en">This ParticipationFunctionality allows to create informative pages with enriched text, images or videos.</rdfs:comment>
        <rdfs:label xml:lang="en">Page</rdfs:label>
    </owl:Class>
    


    <!-- http://ontology.decidim.org/decidim_roadmap/ParticipationArtifact -->

    <owl:Class rdf:about="http://ontology.decidim.org/decidim_roadmap/ParticipationArtifact">
        <rdfs:comment xml:lang="en">General class including the various elements that allow democratic participation in Decidim: ParticipationPlatforms, ParticipationSpaces (such as Participation processes or Assemblies), ParticipationFunctionalities (such as Debates, Surveys or Votations), and ParticipationItems (such as individual proposals, meetings or comments).</rdfs:comment>
        <rdfs:label xml:lang="en">Artifact</rdfs:label>
    </owl:Class>
    


    <!-- http://ontology.decidim.org/decidim_roadmap/ParticipationFunctionality -->

    <owl:Class rdf:about="http://ontology.decidim.org/decidim_roadmap/ParticipationFunctionality">
        <rdfs:subClassOf rdf:resource="http://ontology.decidim.org/decidim_roadmap/ParticipationArtifact"/>
        <rdfs:subClassOf>
            <owl:Restriction>
                <owl:onProperty rdf:resource="http://ontology.decidim.org/decidim_roadmap/functionality_of"/>
                <owl:someValuesFrom rdf:resource="http://ontology.decidim.org/decidim_roadmap/#ParticipationSpace"/>
            </owl:Restriction>
        </rdfs:subClassOf>
        <rdfs:subClassOf>
            <owl:Restriction>
                <owl:onProperty rdf:resource="http://ontology.decidim.org/decidim_roadmap/has_configurator"/>
                <owl:someValuesFrom rdf:resource="http://ontology.decidim.org/decidim_roadmap/Configurator"/>
            </owl:Restriction>
        </rdfs:subClassOf>
        <rdfs:comment xml:lang="en">This class includes the different functionalitites that can be added to a ParticipationSpace by RegisteredParticipants having administrative role to configure it. 

Each ParticipationFunctionality has to be linked to at least one participationSpace it belongs to, through the property functionality_of.
Furthermore, a ParticipationFunctionality needs to have a Configurator that allows its configuration by participants having the permissions to do so.

Some functionalitites represent one single element that is added to the ParticipationSpace, such as a Page, a Votation or a Survey, while other functionalities are elements that contain participationItems, such as Proposals, BudgetedProposals, Meetings or Comments; such functionalitties that contain ParticipationItems are defined as ParticipationContainers.

While some functionalities are general and can belong to any kind of ParticipationSpace, such as a Page, a Blog or a Debate, other are specific to a certain kind of participationSpace. E.g., a WorkingGroup can only belong to an Assembly. In the latter case, the range of the property functionality_of for that particular ParticipationFunctionality is restrictetd to the kind of space it can belong to.</rdfs:comment>
        <rdfs:label xml:lang="en">Component</rdfs:label>
    </owl:Class>
    


    <!-- http://ontology.decidim.org/decidim_roadmap/ParticipationItem -->

    <owl:Class rdf:about="http://ontology.decidim.org/decidim_roadmap/ParticipationItem">
        <rdfs:subClassOf rdf:resource="http://ontology.decidim.org/decidim_roadmap/ParticipationArtifact"/>
        <rdfs:comment xml:lang="en">This general class represents all individual items within a participation space such as Proposals, Comments, meetings, Blog posts.

Items are typically contained in some ParticipationContainer associated with a ParticipationSpace, and different kinds of Items are typically contained in different kinds of containers. For example, Bog posts in Blogs, Proposals in ProposalContainers, Meetings in Workshops or MeetingCalendars, and so on.</rdfs:comment>
        <rdfs:label xml:lang="en">Resource</rdfs:label>
    </owl:Class>
    


    <!-- http://ontology.decidim.org/decidim_roadmap/ParticipationPlatform -->

    <owl:Class rdf:about="http://ontology.decidim.org/decidim_roadmap/ParticipationPlatform">
        <rdfs:subClassOf rdf:resource="http://ontology.decidim.org/decidim_roadmap/ParticipationArtifact"/>
        <rdfs:subClassOf>
            <owl:Restriction>
                <owl:onProperty rdf:resource="http://ontology.decidim.org/decidim_roadmap/has_promoter"/>
                <owl:someValuesFrom rdf:resource="http://ontology.decidim.org/decidim_roadmap/SovereignOrganization"/>
            </owl:Restriction>
        </rdfs:subClassOf>
        <rdfs:comment xml:lang="en">This class represent instances of a participation platform. 

It can include different kinds of ParticipationSpaces, such as Assemblies, Processes, Consultations or Initiatives; all ParticipationArtifacts ultimately relate to some platform.</rdfs:comment>
        <rdfs:label xml:lang="en">Platform</rdfs:label>
    </owl:Class>
    


    <!-- http://ontology.decidim.org/decidim_roadmap/ParticipativeBudget -->

    <owl:Class rdf:about="http://ontology.decidim.org/decidim_roadmap/ParticipativeBudget">
        <rdfs:subClassOf rdf:resource="http://ontology.decidim.org/decidim_roadmap/Container"/>
        <rdfs:subClassOf>
            <owl:Restriction>
                <owl:onProperty rdf:resource="http://ontology.decidim.org/decidim_roadmap/container_of"/>
                <owl:someValuesFrom rdf:resource="http://ontology.decidim.org/decidim_roadmap/BudgetedProject"/>
            </owl:Restriction>
        </rdfs:subClassOf>
        <rdfs:comment xml:lang="en">This component allows participants to collectively define a budget by prioritizing budgeted projects.

It is a ParticipationFunctionality of kind Container, and includes Items of kind BudgetedProposal.</rdfs:comment>
        <rdfs:label xml:lang="en">Participative budget</rdfs:label>
    </owl:Class>
    


    <!-- http://ontology.decidim.org/decidim_roadmap/ParticipativeText -->

    <owl:Class rdf:about="http://ontology.decidim.org/decidim_roadmap/ParticipativeText">
        <rdfs:subClassOf rdf:resource="http://ontology.decidim.org/decidim_roadmap/ProposalContainer"/>
        <rdfs:comment xml:lang="en">This functionality allows participants to collaboratively redact a text as a collection of Proposals. Collaborative editing emerges from interaction of participants with the Proposals that compose the text. 

This functionality is a special kind of ProposalContainer, that composes proposals within a unified text, or decomposes a text into various proposals that can be discussed and prioritized separately.

A ParticipativeText is a Functionality of kind Container, that includes Items of kind Proposal.</rdfs:comment>
        <rdfs:label xml:lang="en">Participative text</rdfs:label>
    </owl:Class>
    


    <!-- http://ontology.decidim.org/decidim_roadmap/Person -->

    <owl:Class rdf:about="http://ontology.decidim.org/decidim_roadmap/Person">
        <rdfs:subClassOf rdf:resource="http://ontology.decidim.org/decidim_roadmap/#Agent"/>
        <rdfs:comment xml:lang="en">General class that represents any person as an individual agent, opposed to collective agents (Organizations).</rdfs:comment>
        <rdfs:label xml:lang="en">Person</rdfs:label>
    </owl:Class>
    


    <!-- http://ontology.decidim.org/decidim_roadmap/Phase -->

    <owl:Class rdf:about="http://ontology.decidim.org/decidim_roadmap/Phase">
        <rdfs:subClassOf rdf:resource="http://ontology.decidim.org/decidim_roadmap/ParticipationFunctionality"/>
        <rdfs:subClassOf>
            <owl:Restriction>
                <owl:onProperty rdf:resource="http://ontology.decidim.org/decidim_roadmap/phase_of"/>
                <owl:qualifiedCardinality rdf:datatype="http://www.w3.org/2001/XMLSchema#nonNegativeInteger">1</owl:qualifiedCardinality>
                <owl:onClass rdf:resource="http://ontology.decidim.org/decidim_roadmap/Process"/>
            </owl:Restriction>
        </rdfs:subClassOf>
        <rdfs:comment xml:lang="en">This functionality allows the administrators of a Process to design and different phases in which the process is divided, with a start and an end date, and with different actions and permissions for each phase.</rdfs:comment>
        <rdfs:label xml:lang="en">Phase</rdfs:label>
    </owl:Class>
    


    <!-- http://ontology.decidim.org/decidim_roadmap/Process -->

    <owl:Class rdf:about="http://ontology.decidim.org/decidim_roadmap/Process">
        <rdfs:subClassOf rdf:resource="http://ontology.decidim.org/decidim_roadmap/#ParticipationSpace"/>
        <rdfs:subClassOf>
            <owl:Restriction>
                <owl:onProperty rdf:resource="http://ontology.decidim.org/decidim_roadmap/has_promoter"/>
                <owl:someValuesFrom rdf:resource="http://ontology.decidim.org/decidim_roadmap/SovereignOrganization"/>
            </owl:Restriction>
        </rdfs:subClassOf>
        <owl:disjointWith rdf:resource="http://ontology.decidim.org/decidim_roadmap/ProcessGroup"/>
        <rdfs:comment xml:lang="en">A Process is a ParticipationSpace that allows participants to interact with one another in different phases in a collective decision making effort.

A Process is promoted by a SovereignOrganization and can contain in different phases different kinds of functionalities, such as Debates, MeetingCalendars, ParticipatoryBudgets or Accountability.</rdfs:comment>
        <rdfs:label xml:lang="en">Process</rdfs:label>
    </owl:Class>
    


    <!-- http://ontology.decidim.org/decidim_roadmap/ProcessGroup -->

    <owl:Class rdf:about="http://ontology.decidim.org/decidim_roadmap/ProcessGroup">
        <rdfs:subClassOf rdf:resource="http://ontology.decidim.org/decidim_roadmap/#ParticipationSpace"/>
        <rdfs:subClassOf>
            <owl:Restriction>
                <owl:onProperty rdf:resource="http://ontology.decidim.org/decidim_roadmap/has_promoter"/>
                <owl:someValuesFrom rdf:resource="http://ontology.decidim.org/decidim_roadmap/SovereignOrganization"/>
            </owl:Restriction>
        </rdfs:subClassOf>
        <rdfs:comment xml:lang="en">A GroupOfProcesses groups together different processes promoted by the same SovereignOrganization.</rdfs:comment>
        <rdfs:label xml:lang="en">Process group</rdfs:label>
    </owl:Class>
    


    <!-- http://ontology.decidim.org/decidim_roadmap/Project -->

    <owl:Class rdf:about="http://ontology.decidim.org/decidim_roadmap/Project">
        <rdfs:subClassOf rdf:resource="http://ontology.decidim.org/decidim_roadmap/ParticipationItem"/>
        <rdfs:subClassOf>
            <owl:Restriction>
                <owl:onProperty rdf:resource="http://ontology.decidim.org/decidim_roadmap/derives_from"/>
                <owl:someValuesFrom rdf:resource="http://ontology.decidim.org/decidim_roadmap/Result"/>
            </owl:Restriction>
        </rdfs:subClassOf>
        <rdfs:comment xml:lang="en">A Project is an Item that represents the implementation of some Result, in turn associated with some accepted Proposal.

It is connected to some Result through the property derived_from, and Participants can monitor its state of execution.</rdfs:comment>
        <rdfs:label xml:lang="en">Project</rdfs:label>
    </owl:Class>
    


    <!-- http://ontology.decidim.org/decidim_roadmap/Promoter -->

    <owl:Class rdf:about="http://ontology.decidim.org/decidim_roadmap/Promoter">
        <rdfs:subClassOf rdf:resource="http://ontology.decidim.org/decidim_roadmap/Role"/>
        <rdfs:comment xml:lang="en">A RegisteredParticipant can have the role of Promoter with respect to a ParticipationArtifact they promote. For example, a SovereignOrganization can be the promoter of a ParticipationPlatform or ParticipationSpace, and a RegisteredParticipant can be the Promoter of an Initiative.</rdfs:comment>
        <rdfs:label xml:lang="en">Promoter</rdfs:label>
    </owl:Class>
    


    <!-- http://ontology.decidim.org/decidim_roadmap/Proposal -->

    <owl:Class rdf:about="http://ontology.decidim.org/decidim_roadmap/Proposal">
        <rdfs:subClassOf rdf:resource="http://ontology.decidim.org/decidim_roadmap/AuthoredItem"/>
        <rdfs:subClassOf>
            <owl:Restriction>
                <owl:onProperty rdf:resource="http://ontology.decidim.org/decidim_roadmap/has_container"/>
                <owl:qualifiedCardinality rdf:datatype="http://www.w3.org/2001/XMLSchema#nonNegativeInteger">1</owl:qualifiedCardinality>
                <owl:onClass rdf:resource="http://ontology.decidim.org/decidim_roadmap/ProposalContainer"/>
            </owl:Restriction>
        </rdfs:subClassOf>
        <rdfs:subClassOf>
            <owl:Restriction>
                <owl:onProperty rdf:resource="http://ontology.decidim.org/decidim_roadmap/has_creator"/>
                <owl:qualifiedCardinality rdf:datatype="http://www.w3.org/2001/XMLSchema#nonNegativeInteger">1</owl:qualifiedCardinality>
                <owl:onClass rdf:resource="http://ontology.decidim.org/decidim_roadmap/#RegisteredParticipant"/>
            </owl:Restriction>
        </rdfs:subClassOf>
        <rdfs:comment xml:lang="en">Proposals are ParticipationItems that can be authored by different kinds of RegisteredParticipants, and can receive support from other VerifiedParticipants. Proposals are moderated and can be rejected, or accepted and turned into Results and Projects.</rdfs:comment>
        <rdfs:label xml:lang="en">Proposal</rdfs:label>
    </owl:Class>
    


    <!-- http://ontology.decidim.org/decidim_roadmap/ProposalContainer -->

    <owl:Class rdf:about="http://ontology.decidim.org/decidim_roadmap/ProposalContainer">
        <rdfs:subClassOf rdf:resource="http://ontology.decidim.org/decidim_roadmap/Container"/>
        <rdfs:subClassOf>
            <owl:Restriction>
                <owl:onProperty rdf:resource="http://ontology.decidim.org/decidim_roadmap/container_of"/>
                <owl:someValuesFrom rdf:resource="http://ontology.decidim.org/decidim_roadmap/Proposal"/>
            </owl:Restriction>
        </rdfs:subClassOf>
        <rdfs:comment xml:lang="en">This functionality allows RegisteredParticipants to create Proposals and comment and support proposals created by others.

It is a ParticipationFunctionality of kind Container, and includes Items of kind Proposal.</rdfs:comment>
        <rdfs:label xml:lang="en">Proposal container</rdfs:label>
    </owl:Class>
    


    <!-- http://ontology.decidim.org/decidim_roadmap/ProposalIncubator -->

    <owl:Class rdf:about="http://ontology.decidim.org/decidim_roadmap/ProposalIncubator">
        <rdfs:subClassOf rdf:resource="http://ontology.decidim.org/decidim_roadmap/Container"/>
        <rdfs:subClassOf>
            <owl:Restriction>
                <owl:onProperty rdf:resource="http://ontology.decidim.org/decidim_roadmap/container_of"/>
                <owl:someValuesFrom rdf:resource="http://ontology.decidim.org/decidim_roadmap/Proposal"/>
            </owl:Restriction>
        </rdfs:subClassOf>
        <rdfs:comment xml:lang="en">A ProposalIncubator allows RegistereParticipants to create Proposal drafts, and collaborate with each other in a preliminary phase before presenting proposals for gathering support to them.

A ProposalIncubator is a Functionality of kind Container, that includes Items of kind &quot;Proposal&quot;.</rdfs:comment>
        <rdfs:label xml:lang="en">Proposal incubator</rdfs:label>
    </owl:Class>
    


    <!-- http://ontology.decidim.org/decidim_roadmap/RegisteredGroup -->

    <owl:Class rdf:about="http://ontology.decidim.org/decidim_roadmap/RegisteredGroup">
        <rdfs:subClassOf rdf:resource="http://ontology.decidim.org/decidim_roadmap/#RegisteredParticipant"/>
        <rdfs:label xml:lang="en">Registered group</rdfs:label>
    </owl:Class>
    


    <!-- http://ontology.decidim.org/decidim_roadmap/RegisteredPerson -->

    <owl:Class rdf:about="http://ontology.decidim.org/decidim_roadmap/RegisteredPerson">
        <rdfs:subClassOf rdf:resource="http://ontology.decidim.org/decidim_roadmap/#RegisteredParticipant"/>
        <rdfs:comment xml:lang="en">A RegisteredParticipant who is an individual Person, as opposed to collective accounts representing Organizations or Groups of participants.</rdfs:comment>
        <rdfs:label xml:lang="en">Registered person</rdfs:label>
    </owl:Class>
    


    <!-- http://ontology.decidim.org/decidim_roadmap/Result -->

    <owl:Class rdf:about="http://ontology.decidim.org/decidim_roadmap/Result">
        <rdfs:subClassOf rdf:resource="http://ontology.decidim.org/decidim_roadmap/ParticipationItem"/>
        <rdfs:subClassOf>
            <owl:Restriction>
                <owl:onProperty rdf:resource="http://ontology.decidim.org/decidim_roadmap/result_of"/>
                <owl:someValuesFrom rdf:resource="http://ontology.decidim.org/decidim_roadmap/Proposal"/>
            </owl:Restriction>
        </rdfs:subClassOf>
        <rdfs:subClassOf>
            <owl:Restriction>
                <owl:onProperty rdf:resource="http://ontology.decidim.org/decidim_roadmap/has_container"/>
                <owl:qualifiedCardinality rdf:datatype="http://www.w3.org/2001/XMLSchema#nonNegativeInteger">1</owl:qualifiedCardinality>
                <owl:onClass rdf:resource="http://ontology.decidim.org/decidim_roadmap/AccountabilityContainer"/>
            </owl:Restriction>
        </rdfs:subClassOf>
        <rdfs:comment xml:lang="en">This kind of ParticipationItem allows Participants to trace and monitor the outcomes of a participative process. 

A Result belongs to an AccountabilityContainer, within a ParticipationSpace.

Each Result is associated to one or more accepted Proposals, and to one or more Projects derived from it. Results are the conjunction between Proposals and Projects that implement them.</rdfs:comment>
        <rdfs:label xml:lang="en">Result</rdfs:label>
    </owl:Class>
    


    <!-- http://ontology.decidim.org/decidim_roadmap/Role -->

    <owl:Class rdf:about="http://ontology.decidim.org/decidim_roadmap/Role">
        <rdfs:subClassOf rdf:resource="http://ontology.decidim.org/decidim_roadmap/Attribute"/>
        <rdfs:subClassOf>
            <owl:Restriction>
                <owl:onProperty rdf:resource="http://ontology.decidim.org/decidim_roadmap/has_scope"/>
                <owl:someValuesFrom rdf:resource="http://ontology.decidim.org/decidim_roadmap/ParticipationArtifact"/>
            </owl:Restriction>
        </rdfs:subClassOf>
        <rdfs:comment xml:lang="en">Abstract class to represent that a given participant has a certain function in the scope of some ParticipationArtifact.</rdfs:comment>
        <rdfs:label xml:lang="en">Role</rdfs:label>
    </owl:Class>
    


    <!-- http://ontology.decidim.org/decidim_roadmap/Scope -->

    <owl:Class rdf:about="http://ontology.decidim.org/decidim_roadmap/Scope">
        <rdfs:subClassOf rdf:resource="http://ontology.decidim.org/decidim_roadmap/Attribute"/>
        <rdfs:comment xml:lang="en">A scope is an Attribute that delimits a ParticipationSpace within a certain geographical area (TerritorialScope subclass) or topic/sector (SectorialScope).</rdfs:comment>
        <rdfs:label xml:lang="en">Scope</rdfs:label>
    </owl:Class>
    


    <!-- http://ontology.decidim.org/decidim_roadmap/SearchEngine -->

    <owl:Class rdf:about="http://ontology.decidim.org/decidim_roadmap/SearchEngine">
        <rdfs:subClassOf rdf:resource="http://ontology.decidim.org/decidim_roadmap/ParticipationFunctionality"/>
        <rdfs:subClassOf>
            <owl:Restriction>
                <owl:onProperty rdf:resource="http://ontology.decidim.org/decidim_roadmap/belong_to"/>
                <owl:qualifiedCardinality rdf:datatype="http://www.w3.org/2001/XMLSchema#nonNegativeInteger">1</owl:qualifiedCardinality>
                <owl:onClass rdf:resource="http://ontology.decidim.org/decidim_roadmap/ParticipationPlatform"/>
            </owl:Restriction>
        </rdfs:subClassOf>
        <rdfs:comment xml:lang="en">A SearchEngine allows participants to search for all the indexable content in a Platform or specific Process or Functionality.</rdfs:comment>
        <rdfs:label xml:lang="en">Search engine</rdfs:label>
    </owl:Class>
    


    <!-- http://ontology.decidim.org/decidim_roadmap/SectorialScope -->

    <owl:Class rdf:about="http://ontology.decidim.org/decidim_roadmap/SectorialScope">
        <rdfs:subClassOf rdf:resource="http://ontology.decidim.org/decidim_roadmap/Scope"/>
        <owl:disjointWith rdf:resource="http://ontology.decidim.org/decidim_roadmap/TerritorialScope"/>
        <rdfs:comment xml:lang="en">A Scope that delimits a ParticipationProcess within a certain topic or sector.</rdfs:comment>
        <rdfs:label xml:lang="en">Sectorial scope</rdfs:label>
    </owl:Class>
    


    <!-- http://ontology.decidim.org/decidim_roadmap/SovereignOrganization -->

    <owl:Class rdf:about="http://ontology.decidim.org/decidim_roadmap/SovereignOrganization">
        <rdfs:subClassOf rdf:resource="http://ontology.decidim.org/decidim_roadmap/Role"/>
        <rdfs:comment xml:lang="en">A SovereignOrganization is the role that an Organization able to take decision and make them effective may assume, promoting a ParticipationPlatform or a ParticipationSpace to involve participants in collective decision making.</rdfs:comment>
        <rdfs:label xml:lang="en">Sovereign organization</rdfs:label>
    </owl:Class>
    


    <!-- http://ontology.decidim.org/decidim_roadmap/Supporter -->

    <owl:Class rdf:about="http://ontology.decidim.org/decidim_roadmap/Supporter">
        <rdfs:subClassOf rdf:resource="http://ontology.decidim.org/decidim_roadmap/Role"/>
        <rdfs:comment xml:lang="en">A registered Participant can have the Role of Supporter with respect to some ParticipationItem they support, such as a Proposal or a BudgetedProposal.</rdfs:comment>
        <rdfs:label xml:lang="en">Supporter</rdfs:label>
    </owl:Class>
    


    <!-- http://ontology.decidim.org/decidim_roadmap/Survey -->

    <owl:Class rdf:about="http://ontology.decidim.org/decidim_roadmap/Survey">
        <rdfs:subClassOf rdf:resource="http://ontology.decidim.org/decidim_roadmap/ParticipationFunctionality"/>
        <rdfs:comment xml:lang="en">This functionality allws Administrators to design, create and configure surveys associated to some ParticipationSpace, with multiple questions that can be answered by RegisteredParticipants.</rdfs:comment>
        <rdfs:label xml:lang="en">Survey</rdfs:label>
    </owl:Class>
    


    <!-- http://ontology.decidim.org/decidim_roadmap/SysAdmin -->

    <owl:Class rdf:about="http://ontology.decidim.org/decidim_roadmap/SysAdmin">
        <rdfs:subClassOf rdf:resource="http://ontology.decidim.org/decidim_roadmap/Administrator"/>
        <rdfs:comment xml:lang="en">A RegisteredParticipant having the role of SysAdmin (Sytem administrator) has rights to access and modify any aspect of the platform. This includes granting any administration role to other RegisteredParticipants.</rdfs:comment>
        <rdfs:label xml:lang="en">Sys admin</rdfs:label>
    </owl:Class>
    


    <!-- http://ontology.decidim.org/decidim_roadmap/TerritorialScope -->

    <owl:Class rdf:about="http://ontology.decidim.org/decidim_roadmap/TerritorialScope">
        <rdfs:subClassOf rdf:resource="http://ontology.decidim.org/decidim_roadmap/Scope"/>
        <rdfs:comment xml:lang="en">A Scope that delimits a ParticipationProcess within a certain geographical area, such as a neighborhood, district, city, province, region or country.</rdfs:comment>
        <rdfs:label xml:lang="en">Territorial scope</rdfs:label>
    </owl:Class>
    


    <!-- http://ontology.decidim.org/decidim_roadmap/Thread -->

    <owl:Class rdf:about="http://ontology.decidim.org/decidim_roadmap/Thread">
        <rdfs:subClassOf rdf:resource="http://ontology.decidim.org/decidim_roadmap/ParticipationItem"/>
        <rdfs:subClassOf>
            <owl:Restriction>
                <owl:onProperty rdf:resource="http://ontology.decidim.org/decidim_roadmap/has_first_comment"/>
                <owl:qualifiedCardinality rdf:datatype="http://www.w3.org/2001/XMLSchema#nonNegativeInteger">1</owl:qualifiedCardinality>
                <owl:onClass rdf:resource="http://ontology.decidim.org/decidim_roadmap/FirstLevelComment"/>
            </owl:Restriction>
        </rdfs:subClassOf>
        <rdfs:comment xml:lang="en">A Thread is ParticipationItem that is composed of different comments, and is started by a FirstLevelComment that opens the conversation.</rdfs:comment>
        <rdfs:label xml:lang="en">Thread</rdfs:label>
    </owl:Class>
    


    <!-- http://ontology.decidim.org/decidim_roadmap/VerifiedGroup -->

    <owl:Class rdf:about="http://ontology.decidim.org/decidim_roadmap/VerifiedGroup">
        <rdfs:subClassOf rdf:resource="http://ontology.decidim.org/decidim_roadmap/RegisteredGroup"/>
        <rdfs:subClassOf rdf:resource="http://ontology.decidim.org/decidim_roadmap/#VerifiedParticipant"/>
        <rdfs:comment xml:lang="en">A Group of Participants whose account has been verified to correspond to the Organization or collective entity it represents.</rdfs:comment>
        <rdfs:label xml:lang="en">Verified group</rdfs:label>
    </owl:Class>
    


    <!-- http://ontology.decidim.org/decidim_roadmap/VerifiedPerson -->

    <owl:Class rdf:about="http://ontology.decidim.org/decidim_roadmap/VerifiedPerson">
        <rdfs:subClassOf rdf:resource="http://ontology.decidim.org/decidim_roadmap/RegisteredPerson"/>
        <rdfs:subClassOf rdf:resource="http://ontology.decidim.org/decidim_roadmap/#VerifiedParticipant"/>
        <rdfs:comment>A RegisteredParticipant whose identity has been verified to correspond to a citizen (or Organization member) with right to vote. Although the identity of a VerifiedParticipant has been verified, it is in general not disclosed; the OfficialAccount subclass represents VerifiedParticipants whose real (verified) identity is publicly disclosed.

Some actions may only be performed by VerifiedPersons, such as supporting a Proposal.</rdfs:comment>
        <rdfs:label xml:lang="en">Verified person</rdfs:label>
    </owl:Class>
    


    <!-- http://ontology.decidim.org/decidim_roadmap/VisitingParticipant -->

    <owl:Class rdf:about="http://ontology.decidim.org/decidim_roadmap/VisitingParticipant">
        <rdfs:subClassOf rdf:resource="http://ontology.decidim.org/decidim_roadmap/#Participant"/>
        <rdfs:comment xml:lang="en">Any participant who visits the platform without logging into a registered account.

Visiting participants can only access content, but cannot modify it or perform actions.</rdfs:comment>
        <rdfs:label xml:lang="en">Visiting participant</rdfs:label>
    </owl:Class>
    


    <!-- http://ontology.decidim.org/decidim_roadmap/Votation -->

    <owl:Class rdf:about="http://ontology.decidim.org/decidim_roadmap/Votation">
        <rdfs:subClassOf rdf:resource="http://ontology.decidim.org/decidim_roadmap/ParticipationFunctionality"/>
        <rdfs:comment xml:lang="en">This functionality represents a votation system associated to a ParticipationSpace.

Different votation systems are possible and can be configured by the Administrators.</rdfs:comment>
        <rdfs:label xml:lang="en">Votation</rdfs:label>
    </owl:Class>
    


    <!-- http://ontology.decidim.org/decidim_roadmap/WorkingGroup -->

    <owl:Class rdf:about="http://ontology.decidim.org/decidim_roadmap/WorkingGroup">
        <rdfs:subClassOf rdf:resource="http://ontology.decidim.org/decidim_roadmap/Group"/>
        <rdfs:subClassOf rdf:resource="http://ontology.decidim.org/decidim_roadmap/ParticipationFunctionality"/>
        <rdfs:subClassOf>
            <owl:Restriction>
                <owl:onProperty rdf:resource="http://ontology.decidim.org/decidim_roadmap/subgroup_of"/>
                <owl:someValuesFrom rdf:resource="http://ontology.decidim.org/decidim_roadmap/Assembly"/>
            </owl:Restriction>
        </rdfs:subClassOf>
        <rdfs:comment xml:lang="en">A WorkingGroup is a Group of participants that collaborate on a specific topic or goal within an Assembly, and interacts with the Assembly it belongs to.</rdfs:comment>
        <rdfs:label xml:lang="en">Working group</rdfs:label>
    </owl:Class>
    


    <!-- http://ontology.decidim.org/decidim_roadmap/Workshop -->

    <owl:Class rdf:about="http://ontology.decidim.org/decidim_roadmap/Workshop">
        <rdfs:subClassOf rdf:resource="http://ontology.decidim.org/decidim_roadmap/Container"/>
        <rdfs:subClassOf>
            <owl:Restriction>
                <owl:onProperty rdf:resource="http://ontology.decidim.org/decidim_roadmap/container_of"/>
                <owl:someValuesFrom rdf:resource="http://ontology.decidim.org/decidim_roadmap/Meeting"/>
            </owl:Restriction>
        </rdfs:subClassOf>
        <rdfs:comment xml:lang="en">A Workshop is a group of meetings with some specific characteristics, such as an interactive descargable program, attendance certificates, videos and materials, and links to coverage of the event in digital media and social media.

A Workshop is a ParticipationFunctionality of kind Container, that includes one or more Meetings.</rdfs:comment>
        <rdfs:label xml:lang="en">Workshop</rdfs:label>
    </owl:Class>
    


    <!-- http://ontology.decidim.org/decidim_roadmap/#Agent -->

    <owl:Class rdf:about="http://ontology.decidim.org/decidim_roadmap/#Agent">
        <rdfs:comment xml:lang="en">An entity that can perform actions. It can be an individual (Person) or a collective (Organization).</rdfs:comment>
        <rdfs:label xml:lang="en">Agent</rdfs:label>
    </owl:Class>
    


    <!-- http://ontology.decidim.org/decidim_roadmap/#Participant -->

    <owl:Class rdf:about="http://ontology.decidim.org/decidim_roadmap/#Participant">
        <rdfs:subClassOf rdf:resource="http://ontology.decidim.org/decidim_roadmap/Role"/>
        <rdfs:comment xml:lang="en">General class that includes any individual or collective entity participating in a participation space</rdfs:comment>
        <rdfs:label xml:lang="en">Participant</rdfs:label>
    </owl:Class>
    


    <!-- http://ontology.decidim.org/decidim_roadmap/#ParticipationSpace -->

    <owl:Class rdf:about="http://ontology.decidim.org/decidim_roadmap/#ParticipationSpace">
        <rdfs:subClassOf rdf:resource="http://ontology.decidim.org/decidim_roadmap/ParticipationArtifact"/>
        <rdfs:subClassOf>
            <owl:Restriction>
                <owl:onProperty rdf:resource="http://ontology.decidim.org/decidim_roadmap/has_configurator"/>
                <owl:someValuesFrom rdf:resource="http://ontology.decidim.org/decidim_roadmap/Configurator"/>
            </owl:Restriction>
        </rdfs:subClassOf>
        <rdfs:subClassOf>
            <owl:Restriction>
                <owl:onProperty rdf:resource="http://ontology.decidim.org/decidim_roadmap/has_promoter"/>
                <owl:someValuesFrom rdf:resource="http://ontology.decidim.org/decidim_roadmap/#Agent"/>
            </owl:Restriction>
        </rdfs:subClassOf>
        <rdfs:subClassOf>
            <owl:Restriction>
                <owl:onProperty rdf:resource="http://ontology.decidim.org/decidim_roadmap/has_scope"/>
                <owl:someValuesFrom rdf:resource="http://ontology.decidim.org/decidim_roadmap/SectorialScope"/>
            </owl:Restriction>
        </rdfs:subClassOf>
        <rdfs:subClassOf>
            <owl:Restriction>
                <owl:onProperty rdf:resource="http://ontology.decidim.org/decidim_roadmap/has_scope"/>
                <owl:someValuesFrom rdf:resource="http://ontology.decidim.org/decidim_roadmap/TerritorialScope"/>
            </owl:Restriction>
        </rdfs:subClassOf>
        <rdfs:subClassOf>
            <owl:Restriction>
                <owl:onProperty rdf:resource="http://ontology.decidim.org/decidim_roadmap/has_platform"/>
                <owl:qualifiedCardinality rdf:datatype="http://www.w3.org/2001/XMLSchema#nonNegativeInteger">1</owl:qualifiedCardinality>
                <owl:onClass rdf:resource="http://ontology.decidim.org/decidim_roadmap/ParticipationPlatform"/>
            </owl:Restriction>
        </rdfs:subClassOf>
        <rdfs:comment xml:lang="en">ParticipationSpaces are the frameworks in which participation takes place. They represent the channels to which the citizens or the members of an organization can articulate collective needs and proposals, and take decisions.

There are different kinds of spaces: Processes, Initiatives, Assemblies, Consultations. Additionally, ProcessGroups are spaces that include and group together more than one Process.

A ParticipationSpace is vinculated to an Agent that promotes it, usually a SovereignOrganization that aims to involve its members or the citizenry in a collective decision making effort. 

A ParticipationSpace is specified by a TerritorialScope and a SectorialScope that delimit its scope.

A ParticipationSpace has some Configurator that allows its configuration and management by RegisteredParticipants having an administrative role that grants them permissions over the ParticipationSpace.</rdfs:comment>
        <rdfs:label xml:lang="en">Space</rdfs:label>
    </owl:Class>
    


    <!-- http://ontology.decidim.org/decidim_roadmap/#RegisteredParticipant -->

    <owl:Class rdf:about="http://ontology.decidim.org/decidim_roadmap/#RegisteredParticipant">
        <rdfs:subClassOf rdf:resource="http://ontology.decidim.org/decidim_roadmap/#Participant"/>
        <rdfs:comment xml:lang="en">A participant corresponding to a registered account in the platform.</rdfs:comment>
        <rdfs:label xml:lang="en">Registered participant</rdfs:label>
    </owl:Class>
    


    <!-- http://ontology.decidim.org/decidim_roadmap/#VerifiedParticipant -->

    <owl:Class rdf:about="http://ontology.decidim.org/decidim_roadmap/#VerifiedParticipant">
        <rdfs:subClassOf rdf:resource="http://ontology.decidim.org/decidim_roadmap/#RegisteredParticipant"/>
        <rdfs:comment>RegisteredParticipant whose account has been verified to correspond to the real world entity it represents, be it an individual person (VerifiedPerson subclass) or a group (VerifiedGroup subclass).</rdfs:comment>
        <rdfs:label xml:lang="en">Verified participant</rdfs:label>
    </owl:Class>
</rdf:RDF>



<!-- Generated by the OWL API (version 4.2.8.20170104-2310) https://github.com/owlcs/owlapi -->
